rt refine RISCV: finish KHeap_R.thy
Signed-off-by: Michael McInerney <m.mcinerney@unsw.edu.au>

proof/refine/RISCV64/KHeap_R.thy
@@ -921,6 +921,8 @@ lemma setObject_in_kernel_mappings[wp]:
   "setObject p val \<lbrace>pspace_in_kernel_mappings'\<rbrace>"
   unfolding pspace_in_kernel_mappings'_def by (unfold_setObject_inmonad)
 
+end
+
 lemma pspace_dom_update:
   "\<lbrakk> ps ptr = Some x; a_type x = a_type v \<rbrakk> \<Longrightarrow> pspace_dom (ps(ptr \<mapsto> v)) = pspace_dom ps"
   apply (simp add: pspace_dom_def dom_fun_upd2 del: dom_fun_upd)
@@ -1826,10 +1828,8 @@ lemma setObject_valid_objs':
 
 lemma setObject_iflive':
   fixes v :: "'a :: pspace_storable"
-  assumes R: "\<And>ko s x y n. (updateObject v ko ptr y n s)
+  assumes R: "\<And>ko s y n. (updateObject v ko ptr y n s)
                    = (updateObject_default v ko ptr y n s)"
-  assumes n: "\<And>x :: 'a. objBits x = n"
-  assumes m: "(1 :: machine_word) < 2 ^ n"
   assumes x: "\<And>x n tcb s t. \<lbrakk> t \<in> fst (updateObject v (KOTCB tcb) ptr x n s); P s;
                                lookupAround2 ptr (ksPSpace s) = (Some (x, KOTCB tcb), n) \<rbrakk>
                   \<Longrightarrow> \<exists>tcb'. t = (KOTCB tcb', s) \<and> (\<forall>(getF, setF) \<in> ran tcb_cte_cases. getF tcb' = getF tcb)"
@@ -2140,24 +2140,6 @@ lemma ex_nonz_cap_to_pres':
                y hoare_vcg_all_lift)
   done
 
-lemma setObject_ksPSpace_only:
-  "\<lbrakk> \<And>p q n ko. \<lbrace>P\<rbrace> updateObject val p q n ko \<lbrace>\<lambda>rv. P \<rbrace>;
-        \<And>f s. P (ksPSpace_update f s) = P s \<rbrakk>
-     \<Longrightarrow> \<lbrace>P\<rbrace> setObject ptr val \<lbrace>\<lambda>rv. P\<rbrace>"
-  apply (simp add: setObject_def split_def)
-  apply (wp | simp | assumption)+
-  done
-
-lemma setObject_ksMachine:
-  "\<lbrakk> \<And>p q n ko. \<lbrace>\<lambda>s. P (ksMachineState s)\<rbrace> updateObject val p q n ko \<lbrace>\<lambda>rv s. P (ksMachineState s)\<rbrace> \<rbrakk>
-     \<Longrightarrow> \<lbrace>\<lambda>s. P (ksMachineState s)\<rbrace> setObject ptr val \<lbrace>\<lambda>rv s. P (ksMachineState s)\<rbrace>"
-  by (simp add: setObject_ksPSpace_only)
-
-lemma setObject_ksInterrupt:
-  "\<lbrakk> \<And>p q n ko. \<lbrace>\<lambda>s. P (ksInterruptState s)\<rbrace> updateObject val p q n ko \<lbrace>\<lambda>rv s. P (ksInterruptState s)\<rbrace> \<rbrakk>
-     \<Longrightarrow> \<lbrace>\<lambda>s. P (ksInterruptState s)\<rbrace> setObject ptr val \<lbrace>\<lambda>rv s. P (ksInterruptState s)\<rbrace>"
-  by (simp add: setObject_ksPSpace_only)
-
 lemma valid_irq_handlers_lift':
   assumes x: "\<And>P. \<lbrace>\<lambda>s. P (cteCaps_of s)\<rbrace> f \<lbrace>\<lambda>rv s. P (cteCaps_of s)\<rbrace>"
   assumes y: "\<And>P. \<lbrace>\<lambda>s. P (ksInterruptState s)\<rbrace> f \<lbrace>\<lambda>rv s. P (ksInterruptState s)\<rbrace>"
@@ -2193,102 +2175,6 @@ lemma valid_arch_state_lift':
    apply (wp typs hoare_vcg_all_lift hoare_vcg_ball_lift arch typ_at_lifts)+
   done
 
-lemma setObject_ep_ct:
-  "\<lbrace>\<lambda>s. P (ksCurThread s)\<rbrace> setObject p (e::endpoint) \<lbrace>\<lambda>_ s. P (ksCurThread s)\<rbrace>"
-  apply (simp add: setObject_def updateObject_ep_eta split_def)
-  apply (wp updateObject_default_inv | simp)+
-  done
-
-lemma setObject_ntfn_ct:
-  "\<lbrace>\<lambda>s. P (ksCurThread s)\<rbrace> setObject p (e::Structures_H.notification)
-   \<lbrace>\<lambda>_ s. P (ksCurThread s)\<rbrace>"
-  apply (simp add: setObject_def split_def)
-  apply (wp updateObject_default_inv | simp)+
-  done
-
-lemma get_ntfn_sp':
-  "\<lbrace>P\<rbrace> getNotification r \<lbrace>\<lambda>t. P and ko_at' t r\<rbrace>"
-  by (clarsimp simp: getNotification_def getObject_def loadObject_default_def
-                     in_monad valid_def obj_at'_def objBits_simps' in_magnitude_check split_def)
-
-lemma set_ntfn_pred_tcb_at' [wp]:
-  "\<lbrace> pred_tcb_at' proj P t \<rbrace>
-   setNotification ep v
-   \<lbrace> \<lambda>rv. pred_tcb_at' proj P t \<rbrace>"
-  apply (simp add: setNotification_def pred_tcb_at'_def)
-  apply (rule obj_at_setObject2)
-  apply (clarsimp simp add: updateObject_default_def in_monad)
-  done
-
-lemma set_ntfn_iflive'[wp]:
-  "\<lbrace>\<lambda>s. if_live_then_nonz_cap' s
-      \<and> (live' (KONotification v) \<longrightarrow> ex_nonz_cap_to' p s)\<rbrace>
-     setNotification p v
-   \<lbrace>\<lambda>rv. if_live_then_nonz_cap'\<rbrace>"
-  apply (simp add: setNotification_def)
-  apply (wp setObject_iflive'[where P="\<top>"])
-       apply simp
-      apply (simp add: objBits_simps)
-     apply (simp add: objBits_simps')
-    apply (clarsimp simp: updateObject_default_def in_monad)
-   apply (clarsimp simp: updateObject_default_def bind_def)
-  apply clarsimp
-  done
-
-declare setNotification_cte_wp_at'[wp]
-
-lemma set_ntfn_cap_to'[wp]:
-  "\<lbrace>ex_nonz_cap_to' p\<rbrace> setNotification p' v \<lbrace>\<lambda>rv. ex_nonz_cap_to' p\<rbrace>"
-  by (wp ex_nonz_cap_to_pres')
-
-lemma setNotification_ifunsafe'[wp]:
-  "\<lbrace>if_unsafe_then_cap'\<rbrace> setNotification p v \<lbrace>\<lambda>rv. if_unsafe_then_cap'\<rbrace>"
-  unfolding setNotification_def
-  apply (rule setObject_ifunsafe'[where P="\<top>", simplified])
-    apply (clarsimp simp: updateObject_default_def in_monad
-                  intro!: equals0I)+
-  apply (simp add: setObject_def split_def)
-  apply (wp updateObject_default_inv | simp)+
-  done
-
-lemma setNotification_idle'[wp]:
-  "\<lbrace>\<lambda>s. valid_idle' s\<rbrace> setNotification p v \<lbrace>\<lambda>rv. valid_idle'\<rbrace>"
-  unfolding setNotification_def
-  apply (wp setObject_idle')
-        apply (simp add: objBits_simps' updateObject_default_inv idle_tcb_ps_def)+
-  done
-
-crunch it[wp]: setNotification "\<lambda>s. P (ksIdleThread s)"
-  (wp: updateObject_default_inv)
-
-lemma set_ntfn_arch' [wp]:
-  "\<lbrace>\<lambda>s. P (ksArchState s)\<rbrace> setNotification ntfn p \<lbrace>\<lambda>_ s. P (ksArchState s)\<rbrace>"
-  apply (simp add: setNotification_def setObject_def split_def)
-  apply (wp updateObject_default_inv|simp)+
-  done
-
-lemma set_ntfn_ksInterrupt[wp]:
-  "\<lbrace>\<lambda>s. P (ksInterruptState s)\<rbrace> setNotification ptr val \<lbrace>\<lambda>rv s. P (ksInterruptState s)\<rbrace>"
-  by (simp add: setNotification_def | wp setObject_ksInterrupt updateObject_default_inv)+
-
-lemma set_ntfn_ksMachine[wp]:
-  "\<lbrace>\<lambda>s. P (ksMachineState s)\<rbrace> setNotification ptr val \<lbrace>\<lambda>rv s. P (ksMachineState s)\<rbrace>"
-  by (simp add: setNotification_def | wp setObject_ksMachine updateObject_default_inv)+
-
-lemma set_ntfn_maxObj [wp]:
-  "\<lbrace>\<lambda>s. P (gsMaxObjectSize s)\<rbrace> setNotification ptr val \<lbrace>\<lambda>rv s. P (gsMaxObjectSize s)\<rbrace>"
-  by (simp add: setNotification_def | wp setObject_ksPSpace_only updateObject_default_inv)+
-
-lemma set_ntfn_global_refs' [wp]:
-  "\<lbrace>valid_global_refs'\<rbrace> setNotification ptr val \<lbrace>\<lambda>_. valid_global_refs'\<rbrace>"
-  by (rule valid_global_refs_lift'; wp)
-
-crunch typ_at' [wp]: setNotification "\<lambda>s. P (typ_at' T p s)" (ignore_del: setObject)
-
-lemma set_ntfn_valid_arch' [wp]:
-  "\<lbrace>valid_arch_state'\<rbrace> setNotification ptr val \<lbrace>\<lambda>_. valid_arch_state'\<rbrace>"
-  by (rule valid_arch_state_lift'; wp)
-
 lemmas valid_irq_node_lift =
     hoare_use_eq_irq_node' [OF _ typ_at_lift_valid_irq_node']
 
@@ -2304,17 +2190,6 @@ lemma valid_irq_states_lift':
   apply (rule hoare_use_eq [where f="\<lambda>s. intStateIRQTable (ksInterruptState s)"], rule x)
   apply wp
   done
-
-lemmas set_ntfn_irq_handlers'[wp] = valid_irq_handlers_lift'' [OF set_ntfn_ctes_of set_ntfn_ksInterrupt]
-
-lemmas set_ntfn_irq_states' [wp] = valid_irq_states_lift' [OF set_ntfn_ksInterrupt set_ntfn_ksMachine]
-
-lemma set_ntfn_vms'[wp]:
-  "\<lbrace>valid_machine_state'\<rbrace> setNotification ptr val \<lbrace>\<lambda>rv. valid_machine_state'\<rbrace>"
-  apply (simp add: setNotification_def valid_machine_state'_def pointerInDeviceData_def pointerInUserData_def)
-  apply (intro hoare_vcg_all_lift hoare_vcg_disj_lift)
-  by (wp setObject_typ_at_inv setObject_ksMachine updateObject_default_inv |
-      simp)+
 
 lemma irqs_masked_lift:
   assumes "\<And>P. \<lbrace>\<lambda>s. P (intStateIRQTable (ksInterruptState s))\<rbrace> f
@@ -2406,6 +2281,8 @@ lemma pspace_aligned'[wp]: "f p v \<lbrace>pspace_aligned'\<rbrace>"
   and pspace_distinct'[wp]: "f p v \<lbrace>pspace_distinct'\<rbrace>"
   and pspace_bounded'[wp]: "f p v \<lbrace>pspace_bounded'\<rbrace>"
   and no_0_obj'[wp]: "f p v \<lbrace>no_0_obj'\<rbrace>"
+  and pspace_canonical'[wp]: "f p v \<lbrace>pspace_canonical'\<rbrace>"
+  and pspace_in_kernel_mappings'[wp]: "f p v \<lbrace>pspace_in_kernel_mappings'\<rbrace>"
   unfolding f_def by (all \<open>wpsimp simp: default_update updateObject_default_def in_monad\<close>)
 
 lemma valid_objs':
@@ -2476,8 +2353,8 @@ lemma setObject_wp:
    setObject ptr (obj :: 'a :: pspace_storable)
    \<lbrace>\<lambda>_. P\<rbrace>"
   apply (wpsimp simp: setObject_def default_update updateObject_default_def fun_upd_def
-                      ARM_H.fromPPtr_def) (* FIXME: arch split *)
-                                          (* FIXME: this is a simp rule, why isn't it available? *)
+                      RISCV64_H.fromPPtr_def) (* FIXME: arch split *)
+                                              (* FIXME: this is a simp rule, why isn't it available? *)
   done
 
 lemmas set_wp = setObject_wp[folded f_def]
@@ -2496,7 +2373,7 @@ lemma setObject_pre:
   supply simps = in_magnitude_check[OF _, unfolded objBits_def] valid_def
                  setObject_def in_monad split_def default_update updateObject_default_def
                  projectKO_eq2 project_inject objBits_def
-                 ARM_H.fromPPtr_def (* FIXME: arch split *)
+                 RISCV64_H.fromPPtr_def (* FIXME: arch split *)
   using assms
   apply (clarsimp simp: simps)
   apply (rename_tac s ko)
@@ -2548,7 +2425,7 @@ lemma getObject_wp:
   "\<lbrace>\<lambda>s. \<forall>ko :: 'a. ko_at' ko p s \<longrightarrow> P ko s\<rbrace>
    getObject p
    \<lbrace>P\<rbrace>"
-  apply (wpsimp simp: getObject_def default_load ARM_H.fromPPtr_def loadObject_default_def
+  apply (wpsimp simp: getObject_def default_load RISCV64_H.fromPPtr_def loadObject_default_def
                       projectKO_def readObject_def omonad_defs split_def)
   apply (rename_tac ko)
   apply (prop_tac "ko_at' ko p s")
@@ -2584,7 +2461,7 @@ lemma getObject_sp:
   "\<lbrace>P\<rbrace> getObject r \<lbrace>\<lambda>rv::'a. P and ko_at' rv r\<rbrace>"
   apply (clarsimp simp: getObject_def loadObject_default_def default_load
                         projectKOs in_monad valid_def obj_at'_def project_inject
-                        split_def ARM_H.fromPPtr_def readObject_def omonad_defs
+                        split_def RISCV64_H.fromPPtr_def readObject_def omonad_defs
                  split: if_split_asm option.split_asm)
   by (clarsimp simp: objBits_def)
 
@@ -3089,33 +2966,6 @@ lemma set_ntfn_iflive'[wp]:
   apply clarsimp
   done
 
-lemma valid_pde_mappings'_def2:
-  "valid_pde_mappings' =
-     (\<lambda>s. \<forall>x. pde_at' x s \<longrightarrow> obj_at' (valid_pde_mapping' (x && mask pdBits)) x s)"
-  apply (clarsimp simp: valid_pde_mappings'_def typ_at_to_obj_at_arches)
-  apply (rule ext, rule iff_allI)
-  apply (clarsimp simp: obj_at'_def projectKOs)
-  apply (auto simp add: objBits_simps archObjSize_def)
-  done
-
-lemma valid_pde_mappings_lift':
-  assumes x: "\<And>P T p. \<lbrace>\<lambda>s. P (typ_at' T p s)\<rbrace> f \<lbrace>\<lambda>rv s. P (typ_at' T p s)\<rbrace>"
-  assumes y: "\<And>x. \<lbrace>obj_at' (valid_pde_mapping' (x && mask pdBits)) x\<rbrace>
-                    f \<lbrace>\<lambda>rv. obj_at' (valid_pde_mapping' (x && mask pdBits)) x\<rbrace>"
-  shows      "\<lbrace>valid_pde_mappings'\<rbrace> f \<lbrace>\<lambda>rv. valid_pde_mappings'\<rbrace>"
-  apply (simp only: valid_pde_mappings'_def2 imp_conv_disj)
-  apply (rule hoare_vcg_all_lift hoare_vcg_disj_lift x y)+
-  done
-
-lemma set_ntfn_valid_pde_mappings'[wp]:
-  "\<lbrace>valid_pde_mappings'\<rbrace> setNotification ptr val \<lbrace>\<lambda>rv. valid_pde_mappings'\<rbrace>"
-  apply (rule valid_pde_mappings_lift')
-   apply wp
-  apply (simp add: setNotification_def)
-  apply (rule obj_at_setObject2)
-  apply (clarsimp simp: updateObject_default_def in_monad)
-  done
-
 end
 
 lemma set_ntfn_minor_invs':
@@ -3219,32 +3069,1807 @@ lemma doMachineOp_invs_bits[wp]:
        | wp cur_tcb_lift sch_act_wf_lift tcb_in_cur_domain'_lift
        | fastforce elim: state_refs_of'_pspaceI)+
 
-crunch obj_at'[wp]: doMachineOp "\<lambda>s. P (obj_at' P' p s)"
+crunches doMachineOp
+  for obj_at'[wp]: "\<lambda>s. P (obj_at' P' p s)"
+  and it[wp]: "\<lambda>s. P (ksIdleThread s)"
+  and idle'[wp]: "valid_idle'"
+  and ko_wp_at'[wp]: "\<lambda>s. P (ko_wp_at' T p s)"
 
-crunch it[wp]: doMachineOp "\<lambda>s. P (ksIdleThread s)"
-crunch idle'[wp]: doMachineOp "valid_idle'"
-  (wp: crunch_wps simp: crunch_simps valid_idle'_pspace_itI)
+context begin interpretation Arch . (*FIXME: arch_split*)
 
-lemma setEndpoint_ksMachine:
-  "\<lbrace>\<lambda>s. P (ksMachineState s)\<rbrace> setEndpoint ptr val \<lbrace>\<lambda>rv s. P (ksMachineState s)\<rbrace>"
-  by (simp add: setEndpoint_def | wp setObject_ksMachine updateObject_default_inv)+
+lemmas bit_simps' = pteBits_def asidHighBits_def asid_low_bits_def
+                    asid_high_bits_def minSchedContextBits_def
+                    replySizeBits_def pageBits_def ptBits_def
 
-lemmas setEndpoint_valid_irq_states'  =
-  valid_irq_states_lift' [OF setEndpoint_ksInterruptState setEndpoint_ksMachine]
+lemmas is_aligned_add_step_le' = is_aligned_add_step_le[simplified mask_2pm1 add_diff_eq]
 
-lemma setEndpoint_ct':
-  "\<lbrace>\<lambda>s. P (ksCurThread s)\<rbrace> setEndpoint a b \<lbrace>\<lambda>rv s. P (ksCurThread s)\<rbrace>"
-  apply (simp add: setEndpoint_def setObject_def split_def)
-  apply (wp updateObject_default_inv | simp)+
+lemma objBitsKO_Data:
+  "objBitsKO (if dev then KOUserDataDevice else KOUserData) = pageBits"
+  by (simp add: objBits_def objBitsKO_def word_size_def)
+
+lemma of_bl_shift_cte_level_bits:
+  "(of_bl z :: machine_word) << cte_level_bits \<le> mask (cte_level_bits + length z)"
+  by word_bitwise
+     (simp add: test_bit_of_bl word_size cte_level_bits_def rev_bl_order_simps)
+
+lemma obj_relation_cuts_range_limit:
+  "\<lbrakk> (p', P) \<in> obj_relation_cuts ko p; P ko ko' \<rbrakk>
+   \<Longrightarrow> \<exists>x n. p' = p + x \<and> is_aligned x n \<and> n \<le> obj_bits ko \<and> x \<le> mask (obj_bits ko)"
+   apply (erule (1) obj_relation_cutsE; clarsimp)
+     apply (drule (1) wf_cs_nD)
+     apply (clarsimp simp: cte_map_def)
+     apply (rule_tac x=cte_level_bits in exI)
+     apply (simp add: is_aligned_shift of_bl_shift_cte_level_bits)
+       apply (rule_tac x=minSchedContextBits in exI)
+       apply (simp add: bit_simps' min_sched_context_bits_def)
+      apply (rule_tac x=replySizeBits in exI)
+      apply (simp add: replySizeBits_def)
+     apply (rule_tac x=pteBits in exI)
+     apply (simp add: bit_simps is_aligned_shift mask_def pteBits_def)
+     apply word_bitwise
+   apply (rule_tac x=pageBits in exI)
+   apply (simp add: is_aligned_shift pbfs_atleast_pageBits is_aligned_mult_triv2)
+   apply (simp add: mask_def shiftl_t2n mult_ac)
+   apply (frule word_less_power_trans2, rule pbfs_atleast_pageBits)
+    apply (simp add: pbfs_less_wb'[unfolded word_bits_def, simplified])
+   apply (simp add: pbfs_less_wb'[unfolded word_bits_def, simplified])
+  apply fastforce
   done
 
-lemmas setEndpoint_valid_globals[wp]
-    = valid_global_refs_lift' [OF set_ep_ctes_of set_ep_arch'
-                                  setEndpoint_it setEndpoint_ksInterruptState]
-lemma obj_at'_is_canonical:
-  "\<lbrakk>pspace_canonical' s; obj_at' P t s\<rbrakk> \<Longrightarrow> canonical_address t"
-  apply (clarsimp simp: obj_at'_def pspace_canonical'_def)
-  by (drule_tac x=t in bspec) clarsimp+
+lemma obj_relation_cuts_range_mask_range:
+  "\<lbrakk> (p', P) \<in> obj_relation_cuts ko p; P ko ko'; is_aligned p (obj_bits ko) \<rbrakk>
+   \<Longrightarrow> p' \<in> mask_range p (obj_bits ko)"
+  apply (drule (1) obj_relation_cuts_range_limit, clarsimp)
+  apply (rule conjI)
+   apply (rule word_plus_mono_right2; assumption?)
+   apply (simp add: is_aligned_no_overflow_mask)
+  apply (erule word_plus_mono_right)
+  apply (simp add: is_aligned_no_overflow_mask)
+  done
+
+lemma obj_relation_cuts_obj_bits:
+  "\<lbrakk> (p', P) \<in> obj_relation_cuts ko p; P ko ko' \<rbrakk> \<Longrightarrow> objBitsKO ko' \<le> obj_bits ko"
+  apply (erule (1) obj_relation_cutsE;
+          clarsimp simp: objBits_simps objBits_defs cte_level_bits_def sc_const_eq[symmetric]
+                         pbfs_atleast_pageBits[simplified bit_simps] archObjSize_def pteBits_def
+                         table_size_def pte_bits_def ptTranslationBits_def pageBits_def)
+  apply (clarsimp simp: scBits_inverse_sc_relation[simplified])
+  apply (cases ko; simp add: other_obj_relation_def objBits_defs
+                      split: kernel_object.splits)
+  apply (rename_tac ako, case_tac ako; clarsimp)
+  apply (rename_tac ako', case_tac ako'; clarsimp simp: archObjSize_def)
+  done
+
+lemma typ_at'_same_type:
+  assumes "typ_at' T p s" "koTypeOf k = koTypeOf ko" "objBitsKO k = objBitsKO ko" "ksPSpace s p' = Some ko"
+  shows "typ_at' T p (s\<lparr>ksPSpace :=ksPSpace s(p' \<mapsto> k)\<rparr>)"
+  using assms
+  by (clarsimp simp: typ_at'_def ko_wp_at'_def ps_clear_upd)
+
+lemma cte_at'_same_type:
+  "\<lbrakk>cte_wp_at' \<top> t s; koTypeOf k = koTypeOf ko;objBitsKO k = objBitsKO ko;
+    ksPSpace s p = Some ko\<rbrakk>
+      \<Longrightarrow> cte_wp_at' \<top> t (s\<lparr>ksPSpace := ksPSpace s(p \<mapsto> k)\<rparr>)"
+  apply (simp add: cte_at_typ' typ_at'_same_type)
+  apply (elim exE disjE)
+   apply (rule disjI1, clarsimp simp: typ_at'_same_type)
+  apply (rule disjI2, rule_tac x=n in exI, clarsimp simp: typ_at'_same_type)
+  done
+
+lemma valid_ep'_ep_update:
+  "\<lbrakk> valid_objs' s; valid_ep' ep s; ep_at' epPtr s; ksPSpace s x = Some (KOEndpoint obj) \<rbrakk>
+     \<Longrightarrow> valid_ep' obj (s\<lparr>ksPSpace := ksPSpace s(epPtr \<mapsto> KOEndpoint ep)\<rparr>)"
+  apply (erule (1) valid_objsE')
+  apply (fastforce simp: valid_objs'_def valid_obj'_def obj_at'_def projectKOs valid_ep'_def
+                  split: endpoint.splits)
+  done
+
+lemma valid_cap'_ep_update:
+  "\<lbrakk> valid_cap' cap s; valid_objs' s; valid_ep' ep s; ep_at' epPtr s \<rbrakk>
+     \<Longrightarrow> valid_cap' cap (s\<lparr>ksPSpace := ksPSpace s(epPtr \<mapsto> KOEndpoint ep)\<rparr>)"
+  supply ps_clear_upd[simp]
+  apply (clarsimp simp: typ_at'_same_type ko_wp_at'_def cte_at'_same_type
+                        valid_cap'_def obj_at'_def projectKOs objBits_simps
+                 split: endpoint.splits capability.splits)
+         apply fastforce+
+       apply (clarsimp split: zombie_type.splits simp: projectKOs obj_at'_def typ_at'_same_type)
+       apply (intro conjI impI; clarsimp)
+        apply (drule_tac x=addr in spec, clarsimp)
+       apply (drule_tac x=addr in spec, clarsimp)
+      apply (clarsimp simp: objBits_simps page_table_at'_def frame_at'_def
+                            valid_arch_cap'_def valid_arch_cap_ref'_def
+                     split: arch_capability.splits  option.splits if_split_asm
+           | rule_tac ko="KOEndpoint obj" in typ_at'_same_type[where p'=epPtr]
+           | simp)+
+     apply fastforce
+    apply (clarsimp simp: valid_untyped'_def ko_wp_at'_def obj_range'_def split: if_split_asm)
+     apply (drule_tac x=epPtr in spec, fastforce simp: objBits_simps)+
+   apply (drule_tac x=addr in spec, fastforce)
+  apply fastforce
+  done
+
+lemma valid_cap'_reply_update:
+  "\<lbrakk> valid_cap' cap s; valid_objs' s; valid_reply' reply s; reply_at' rptr s \<rbrakk>
+     \<Longrightarrow> valid_cap' cap (s\<lparr>ksPSpace := ksPSpace s(rptr \<mapsto> KOReply reply)\<rparr>)"
+  supply ps_clear_upd[simp]
+  apply (clarsimp simp: typ_at'_same_type ko_wp_at'_def cte_at'_same_type
+                        valid_cap'_def obj_at'_def projectKOs objBits_simps
+                 split: endpoint.splits capability.splits)
+         apply fastforce+
+      apply (clarsimp split: zombie_type.splits simp: projectKOs obj_at'_def typ_at'_same_type)
+      apply (intro conjI impI; clarsimp)
+       apply (drule_tac x=addr in spec, clarsimp)
+      apply (drule_tac x=addr in spec, clarsimp)
+     apply (clarsimp simp: objBits_simps page_table_at'_def frame_at'_def
+                           valid_arch_cap'_def valid_arch_cap_ref'_def
+                    split: arch_capability.splits  option.splits if_split_asm
+          | rule_tac ko="KOReply obj" in typ_at'_same_type[where p'=rptr])+
+    apply (clarsimp simp: valid_untyped'_def ko_wp_at'_def obj_range'_def split: if_split_asm)
+     apply (drule_tac x=rptr in spec, fastforce simp: objBits_simps)+
+   apply (drule_tac x=addr in spec, fastforce)
+  apply fastforce
+  done
+
+lemma valid_tcb_state'_ep_update:
+  "\<lbrakk> valid_objs' s; valid_ep' ep s; ep_at' epPtr s;  ksPSpace s x = Some (KOTCB obj) \<rbrakk>
+     \<Longrightarrow> valid_tcb_state' (tcbState obj) (s\<lparr>ksPSpace := ksPSpace s(epPtr \<mapsto> KOEndpoint ep)\<rparr>)"
+  apply (rule valid_objsE', simp, simp)
+  by (fastforce simp: typ_at'_same_type ps_clear_upd objBits_simps valid_obj'_def projectKOs
+                      valid_tcb_state'_def valid_bound_obj'_def valid_tcb'_def obj_at'_def
+               split: option.splits thread_state.splits)
+
+lemma valid_tcb_state'_reply_update:
+  "\<lbrakk> valid_objs' s; valid_reply' reply s; reply_at' rptr s; ksPSpace s x = Some (KOTCB obj) \<rbrakk>
+     \<Longrightarrow> valid_tcb_state' (tcbState obj) (s\<lparr>ksPSpace := ksPSpace s(rptr \<mapsto> KOReply reply)\<rparr>)"
+  apply (rule valid_objsE', simp, simp)
+  by (fastforce simp: typ_at'_same_type ps_clear_upd objBits_simps valid_obj'_def projectKOs
+                      valid_bound_obj'_def valid_tcb'_def valid_tcb_state'_def obj_at'_def
+               split: option.splits thread_state.splits)
+
+lemma valid_tcb'_ep_update:
+  "\<lbrakk> valid_objs' s; valid_ep' ep s; ep_at' epPtr s; ksPSpace s x = Some (KOTCB obj) \<rbrakk>
+     \<Longrightarrow> valid_tcb' obj (s\<lparr>ksPSpace := ksPSpace s(epPtr \<mapsto> KOEndpoint ep)\<rparr>)"
+  apply (rule valid_objsE', simp, simp)
+  by (fastforce simp: typ_at'_same_type ps_clear_upd objBits_simps valid_obj'_def projectKOs
+                      valid_bound_obj'_def valid_tcb'_def obj_at'_def valid_tcb_state'_ep_update
+                      valid_cap'_ep_update
+              split: option.splits thread_state.splits)
 
 end
+
+lemma valid_obj'_ep_update:
+  "\<lbrakk> valid_objs' s; valid_ep' ep s; ep_at' epPtr s; ksPSpace s x = Some obj\<rbrakk>
+       \<Longrightarrow> valid_obj' obj (s\<lparr>ksPSpace := ksPSpace s(epPtr \<mapsto> KOEndpoint ep)\<rparr>)"
+  apply (rule valid_objsE', simp, simp)
+  by (cases obj;
+      clarsimp simp: typ_at'_same_type valid_obj'_def obj_at'_def ps_clear_upd
+                     valid_ntfn'_def  valid_bound_obj'_def valid_reply'_def valid_cte'_def
+                     valid_sched_context'_def objBits_simps projectKOs valid_cap'_ep_update
+                     valid_ep'_ep_update valid_tcb'_ep_update
+              split: endpoint.splits ntfn.splits option.splits)
+     fastforce+
+
+lemma valid_obj'_reply_update:
+  "\<lbrakk> valid_objs' s; valid_reply' reply s; reply_at' rptr s; ksPSpace s x = Some obj \<rbrakk>
+     \<Longrightarrow> valid_obj' obj (s\<lparr>ksPSpace := ksPSpace s(rptr \<mapsto> KOReply reply)\<rparr>)"
+  apply (rule valid_objsE', simp, simp)
+  apply (cases obj; clarsimp simp: valid_obj'_def)
+       apply (fastforce simp: valid_ep'_def obj_at'_def projectKOs split: endpoint.split)
+      apply (fastforce simp: valid_bound_obj'_def valid_ntfn'_def obj_at'_def projectKOs
+                      split: ntfn.splits option.split)
+     apply (fastforce simp: valid_bound_obj'_def valid_tcb'_def valid_tcb_state'_reply_update
+                            valid_cap'_reply_update obj_at'_def projectKOs tcb_cte_cases_def
+                     split: option.split)
+    apply (fastforce simp: valid_cap'_reply_update obj_at'_def valid_cte'_def projectKOs)
+   apply (fastforce simp: valid_sched_context'_def valid_bound_obj'_def objBitsKO_def
+                          obj_at'_def projectKOs ps_clear_upd
+                   split: option.split)
+  apply (fastforce simp: valid_reply'_def valid_bound_obj'_def obj_at'_def projectKOs objBitsKO_def
+                  split: option.split)
+  done
+
+lemma valid_objs'_ep_update:
+  "\<lbrakk> valid_objs' s; valid_ep' ep s; ep_at' epPtr s \<rbrakk>
+     \<Longrightarrow> valid_objs' (s\<lparr>ksPSpace := ksPSpace s(epPtr \<mapsto> KOEndpoint ep)\<rparr>)"
+  apply (clarsimp simp: valid_objs'_def obj_at'_def projectKOs)
+  apply (erule ranE)
+  apply (clarsimp simp: ps_clear_upd split: if_split_asm)
+   apply (fastforce simp: valid_obj'_def valid_ep'_def obj_at'_def ps_clear_upd
+                          objBits_simps projectKOs
+                   split: endpoint.splits)
+  apply (fastforce intro!: valid_obj'_ep_update simp: valid_objs'_def obj_at'_def projectKOs)
+  done
+
+lemma valid_objs'_reply_update:
+  "\<lbrakk> valid_objs' s; valid_reply' reply s; reply_at' rptr s \<rbrakk>
+     \<Longrightarrow> valid_objs' (s\<lparr>ksPSpace := ksPSpace s(rptr \<mapsto> KOReply reply)\<rparr>)"
+  apply (clarsimp simp: valid_objs'_def obj_at'_def projectKOs)
+  apply (erule ranE)
+  apply (clarsimp split: if_split_asm)
+   apply (fastforce simp: valid_bound_obj'_def valid_obj'_def valid_reply'_def
+                          obj_at'_def projectKOs objBitsKO_def
+                   split: option.splits)
+  apply (fastforce intro!: valid_obj'_reply_update simp: valid_objs'_def obj_at'_def projectKOs)
+  done
+
+lemma valid_release_queue_ksPSpace_update:
+  "\<lbrakk>valid_release_queue s;
+    ko_wp_at' (\<lambda>ko'. koTypeOf ko' = koTypeOf ko \<and> objBitsKO ko' = objBitsKO ko) ptr s;
+    koTypeOf ko \<noteq> TCBT\<rbrakk> \<Longrightarrow>
+    valid_release_queue (s\<lparr>ksPSpace := ksPSpace s(ptr \<mapsto> ko)\<rparr>)"
+  by (fastforce simp: valid_release_queue_def ko_wp_at'_def obj_at'_def projectKOs ps_clear_upd)
+
+lemma valid_release_queue'_ksPSpace_update:
+  "\<lbrakk>valid_release_queue' s;
+    ko_wp_at' (\<lambda>ko'. koTypeOf ko' = koTypeOf ko \<and> objBitsKO ko' = objBitsKO ko) ptr s;
+    koTypeOf ko \<noteq> TCBT\<rbrakk> \<Longrightarrow>
+    valid_release_queue' (s\<lparr>ksPSpace := ksPSpace s(ptr \<mapsto> ko)\<rparr>)"
+  by (fastforce simp: valid_release_queue'_def ko_wp_at'_def obj_at'_def projectKOs ps_clear_upd)
+
+lemma sym_ref_Receive_or_Reply_replyTCB':
+  "\<lbrakk> sym_refs (state_refs_of' s); ko_at' tcb tp s;
+     tcbState tcb = BlockedOnReceive ep pl (Some rp)
+     \<or> tcbState tcb = BlockedOnReply (Some rp) \<rbrakk> \<Longrightarrow>
+    \<exists>reply. ksPSpace s rp = Some (KOReply reply) \<and> replyTCB reply = Some tp"
+  apply (drule (1) sym_refs_obj_atD'[rotated, where p=tp])
+  apply (clarsimp simp: state_refs_of'_def projectKOs obj_at'_def)
+  apply (clarsimp simp: ko_wp_at'_def)
+  apply (erule disjE; clarsimp)
+  apply (rename_tac koa; case_tac koa;
+         simp add: get_refs_def2 ep_q_refs_of'_def ntfn_q_refs_of'_def
+                   tcb_st_refs_of'_def tcb_bound_refs'_def
+            split: endpoint.split_asm ntfn.split_asm thread_state.split_asm if_split_asm)+
+  done
+
+lemma sym_ref_replyTCB_Receive_or_Reply:
+  "\<lbrakk> ko_at' reply rp s; sym_refs (state_refs_of' s); replyTCB reply = Some tp \<rbrakk>
+   \<Longrightarrow> st_tcb_at' (\<lambda>st. (\<exists>ep pl. st = BlockedOnReceive ep pl (Some rp))
+                        \<or> st = BlockedOnReply (Some rp)) tp s"
+  apply (drule (1) sym_refs_obj_atD'[rotated, where p=rp])
+  apply (clarsimp simp: state_refs_of'_def projectKOs pred_tcb_at'_def obj_at'_def)
+  apply (clarsimp simp: ko_wp_at'_def)
+  apply (rename_tac tcb; case_tac tcb;
+         simp add: get_refs_def2 ntfn_q_refs_of'_def
+                   tcb_st_refs_of'_def tcb_bound_refs'_def
+            split: ntfn.split_asm thread_state.split_asm)+
+  done
+
+lemma sym_ref_BlockedOnSend_SendEP':
+  "\<lbrakk> sym_refs (state_refs_of' s); st_tcb_at' ((=) (BlockedOnSend eptr p1 p2 p3 p4)) tp s\<rbrakk>
+      \<Longrightarrow> \<exists>list. ko_wp_at' ((=) (KOEndpoint (SendEP list))) eptr s"
+  apply (simp add: pred_tcb_at'_def)
+  apply (drule (1) sym_refs_obj_atD'[rotated, where p=tp])
+  apply (clarsimp simp: state_refs_of'_def projectKOs obj_at'_def)
+  apply (drule sym[where s="BlockedOnSend _ _ _ _ _"])
+  apply (clarsimp simp: ko_wp_at'_def)
+  apply (rename_tac ko; case_tac ko;
+         simp add: get_refs_def2 ep_q_refs_of'_def ntfn_q_refs_of'_def
+                   tcb_st_refs_of'_def tcb_bound_refs'_def
+            split: endpoint.split_asm ntfn.split_asm thread_state.split_asm if_split_asm)+
+  done
+
+lemma sym_ref_BlockedOnReceive_RecvEP':
+  "\<lbrakk> sym_refs (state_refs_of' s); st_tcb_at' ((=) (BlockedOnReceive eptr pl ropt)) tp s\<rbrakk>
+     \<Longrightarrow> \<exists>list. ko_wp_at' ((=) (KOEndpoint (RecvEP list))) eptr s"
+  apply (simp add: pred_tcb_at'_def)
+  apply (drule (1) sym_refs_obj_atD'[rotated, where p=tp])
+  apply (clarsimp simp: state_refs_of'_def projectKOs obj_at'_def)
+  apply (drule sym[where s="BlockedOnReceive _ _ _"])
+  apply (clarsimp simp: ko_wp_at'_def split: if_split_asm)
+   apply (rename_tac ko koa; case_tac ko;
+          simp add: get_refs_def2 ep_q_refs_of'_def ntfn_q_refs_of'_def
+                    tcb_st_refs_of'_def tcb_bound_refs'_def
+             split: endpoint.split_asm ntfn.split_asm thread_state.split_asm if_split_asm)
+  apply (rename_tac ko; case_tac ko;
+         simp add: get_refs_def2 ep_q_refs_of'_def ntfn_q_refs_of'_def
+                   tcb_st_refs_of'_def tcb_bound_refs'_def
+            split: endpoint.split_asm ntfn.split_asm thread_state.split_asm if_split_asm)
+  done
+
+lemma Receive_or_Send_ep_at':
+  "\<lbrakk> st = BlockedOnReceive epPtr pl rp \<or> st = BlockedOnSend epPtr p1 p2 p3 p4;
+     valid_objs' s; st_tcb_at' ((=) st) t s\<rbrakk>
+       \<Longrightarrow> ep_at' epPtr s"
+  apply (drule (1) tcb_in_valid_state')
+  by (fastforce simp: obj_at'_def valid_tcb_state'_def)
+
+lemma ep_queued_st_tcb_at':
+  "\<And>P. \<lbrakk>ko_at' ep ptr s; \<exists>rt. (t, rt) \<in> ep_q_refs_of' ep;
+         valid_objs' s; sym_refs (state_refs_of' s);
+         \<And>bo bbadge bgrant breply bcall r. P (Structures_H.BlockedOnSend bo bbadge bgrant breply bcall) \<and>
+                         P (Structures_H.BlockedOnReceive bo bgrant r) \<rbrakk>
+    \<Longrightarrow> st_tcb_at' P t s"
+  apply (case_tac ep, simp_all)
+  apply (frule(1) sym_refs_ko_atD', clarsimp, erule (1) my_BallE,
+         clarsimp simp: pred_tcb_at'_def refs_of_rev' obj_at'_def ko_wp_at'_def projectKOs)+
+  done
+
+(* cross lemmas *)
+
+context begin interpretation Arch . (*FIXME: arch_split*)
+
+lemma pspace_aligned_cross:
+  "\<lbrakk> pspace_aligned s; pspace_relation (kheap s) (ksPSpace s') \<rbrakk> \<Longrightarrow> pspace_aligned' s'"
+  apply (clarsimp simp: pspace_aligned'_def pspace_aligned_def pspace_relation_def)
+  apply (rename_tac p' ko')
+  apply (prop_tac "p' \<in> pspace_dom (kheap s)", fastforce)
+  apply (thin_tac "pspace_dom k = p" for k p)
+  apply (clarsimp simp: pspace_dom_def)
+  apply (drule bspec, fastforce)+
+  apply clarsimp
+  apply (rename_tac ko' a a' P ko)
+  apply (erule (1) obj_relation_cutsE; clarsimp simp: objBits_simps)
+
+  \<comment>\<open>CNode\<close>
+     apply (clarsimp simp: cte_map_def)
+     apply (simp only: cteSizeBits_def cte_level_bits_def)
+     apply (rule is_aligned_add)
+      apply (erule is_aligned_weaken, simp)
+     apply (rule is_aligned_weaken)
+    apply (rule is_aligned_shiftl_self, simp)
+
+  \<comment>\<open>SchedContext, Reply\<close>
+     apply ((clarsimp simp: minSchedContextBits_def min_sched_context_bits_def replySizeBits_def
+                            scBits_inverse_sc_relation[simplified]
+                     elim!: is_aligned_weaken)+)[2]
+
+  \<comment>\<open>PageTable\<close>
+   apply (clarsimp simp: archObjSize_def pteBits_def table_size_def ptTranslationBits_def pte_bits_def)
+    apply (rule is_aligned_add)
+     apply (erule is_aligned_weaken)
+     apply simp
+    apply (rule is_aligned_shift)
+
+
+  \<comment>\<open>DataPage\<close>
+   apply (rule is_aligned_add)
+    apply (erule is_aligned_weaken)
+    apply (clarsimp simp: pageBitsForSize_def)
+    apply (case_tac sz; simp add: pageBits_def)
+    apply (rule is_aligned_shiftl_self)
+
+  \<comment>\<open>other_obj_relation\<close>
+  apply (simp add: other_obj_relation_def)
+  apply (clarsimp simp: bit_simps' tcbBlockSizeBits_def epSizeBits_def ntfnSizeBits_def
+              split: kernel_object.splits Structures_A.kernel_object.splits)
+  apply (fastforce simp: archObjSize_def split: arch_kernel_object.splits arch_kernel_obj.splits)
+  done
+
+lemma pspace_relation_pspace_bounded':
+  "\<lbrakk> pspace_relation (kheap s) (ksPSpace s') \<rbrakk> \<Longrightarrow> pspace_bounded' s'"
+  apply (clarsimp simp: pspace_bounded'_def pspace_relation_def)
+  apply (rename_tac p' ko')
+  apply (prop_tac "p' \<in> pspace_dom (kheap s)", fastforce)
+  apply (thin_tac "pspace_dom k = p" for k p)
+  apply (clarsimp simp: pspace_dom_def)
+  apply (drule bspec, fastforce)+
+  apply clarsimp
+  apply (rename_tac ko' a a' P ko)
+  apply (erule (1) obj_relation_cutsE;
+         clarsimp simp: objBits_simps' word_bits_def pageBits_def archObjSize_def pteBits_def)
+
+  \<comment>\<open>SchedContext\<close>
+     apply (clarsimp simp: minSchedContextBits_def min_sched_context_bits_def replySizeBits_def
+                            scBits_inverse_sc_relation[simplified] valid_sched_context_size_def
+                            untyped_max_bits_def
+                     elim!: is_aligned_weaken)
+
+  \<comment>\<open>other_obj_relation\<close>
+  apply (simp add: other_obj_relation_def)
+  by (clarsimp simp: bit_simps' tcbBlockSizeBits_def epSizeBits_def ntfnSizeBits_def
+              split: kernel_object.splits Structures_A.kernel_object.splits)
+     (clarsimp simp: archObjSize_def pteBits_def pageBits_def
+              split: arch_kernel_object.splits arch_kernel_obj.splits)
+
+lemma pspace_distinct_cross:
+  "\<lbrakk> pspace_distinct s; pspace_aligned s; pspace_relation (kheap s) (ksPSpace s') \<rbrakk> \<Longrightarrow>
+   pspace_distinct' s'"
+  apply (frule (1) pspace_aligned_cross)
+  apply (clarsimp simp: pspace_distinct'_def)
+  apply (rename_tac p' ko')
+  apply (rule pspace_dom_relatedE; assumption?)
+  apply (rename_tac p ko P)
+  apply (frule (1) pspace_alignedD')
+  apply (frule (1) pspace_alignedD)
+  apply (frule pspace_relation_pspace_bounded')
+    apply (frule (1) pspace_boundedD')
+  apply (rule ps_clearI, assumption)
+   apply (case_tac ko'; simp add: objBits_simps objBits_defs bit_simps' scBits_pos_power2)
+   apply (clarsimp split: arch_kernel_object.splits simp: bit_simps' archObjSize_def)
+  apply (rule ccontr, clarsimp)
+  apply (rename_tac x' ko_x')
+  apply (frule_tac x=x' in pspace_alignedD', assumption)
+  apply (rule_tac x=x' in pspace_dom_relatedE; assumption?)
+  apply (rename_tac x ko_x P')
+  apply (frule_tac p=x in pspace_alignedD, assumption)
+  apply (case_tac "p = x")
+   apply clarsimp
+   apply (erule (1) obj_relation_cutsE; clarsimp)
+      apply (clarsimp simp: cte_relation_def cte_map_def objBits_simps)
+      apply (rule_tac n=cteSizeBits in is_aligned_add_step_le'; assumption?)
+     apply (clarsimp simp: pte_relation_def objBits_simps archObjSize_def)
+     apply (rule_tac n=pteBits in is_aligned_add_step_le'; assumption?)
+    apply (simp add: objBitsKO_Data)
+    apply (rule_tac n=pageBits in is_aligned_add_step_le'; assumption?)
+   apply (case_tac ko;
+          simp split: if_split_asm
+                 add: is_other_obj_relation_type_CapTable
+                      is_other_obj_relation_type_SchedContext
+                      is_other_obj_relation_type_Reply
+                      a_type_def)
+   apply (rename_tac ako,
+          case_tac ako;
+          simp add: is_other_obj_relation_type_def a_type_def split: if_split_asm)
+  apply (frule (1) obj_relation_cuts_obj_bits)
+  apply (drule (2) obj_relation_cuts_range_mask_range)+
+  apply (prop_tac "x' \<in> mask_range p' (objBitsKO ko')", simp add: mask_def add_diff_eq)
+  apply (frule_tac x=p and y=x in pspace_distinctD; assumption?)
+  apply (drule (4) mask_range_subsetD)
+  apply (erule (2) in_empty_interE)
+  done
+
+lemma aligned'_distinct'_ko_at'I:
+  "\<lbrakk>ksPSpace s' x = Some ko;  pspace_aligned' s'; pspace_distinct' s';
+    (if koTypeOf ko  = SchedContextT then pspace_bounded' s' else True);
+    ko = injectKO (v:: 'a :: pspace_storable)\<rbrakk>
+      \<Longrightarrow> ko_at' v x s'"
+  apply (simp add: obj_at'_def projectKOs project_inject pspace_bounded'_def
+                   pspace_distinct'_def pspace_aligned'_def)
+  apply (drule bspec, erule domI)+
+  apply (case_tac "injectKO v"; clarsimp simp: valid_sz_simps dest!: pspace_boundedD')
+  done
+
+lemma aligned_distinct_ko_at'I:
+  assumes p: "pspace_relation (kheap s) (ksPSpace s')"
+  assumes ps: "pspace_aligned s" "pspace_distinct s"
+  shows "\<lbrakk>ksPSpace s' x = Some ko; ko = injectKO (v:: 'a :: pspace_storable)\<rbrakk>
+      \<Longrightarrow> ko_at' v x s'"
+  apply (rule aligned'_distinct'_ko_at'I[OF _ pspace_aligned_cross[OF ps(1) p]]; simp)
+  using assms by (fastforce dest!: pspace_distinct_cross simp: pspace_relation_pspace_bounded'[OF p])+
+
+lemma tcb_at_cross:
+  assumes p: "pspace_relation (kheap s) (ksPSpace s')"
+  assumes aligned: "pspace_aligned s"
+  assumes distinct: "pspace_distinct s"
+  assumes t: "tcb_at t s"
+  shows "tcb_at' t s'" using assms
+  apply (clarsimp simp: obj_at_def is_tcb)
+  apply (drule (1) pspace_relation_absD, clarsimp simp: other_obj_relation_def)
+  apply (case_tac z; simp)
+  by (fastforce dest!: aligned_distinct_ko_at'I[where 'a=tcb] elim: obj_at'_weakenE)
+
+lemma st_tcb_at_coerce_abstract:
+  assumes t: "st_tcb_at' P t c"
+  assumes sr: "(a, c) \<in> state_relation"
+  shows "st_tcb_at (\<lambda>st. \<exists>st'. thread_state_relation st st' \<and> P st') t a"
+  using assms
+  apply (clarsimp simp: state_relation_def pred_tcb_at'_def obj_at'_def
+                        projectKOs)
+  apply (erule (1) pspace_dom_relatedE)
+  apply (erule (1) obj_relation_cutsE, simp_all)
+  apply (clarsimp simp: st_tcb_at_def obj_at_def other_obj_relation_def
+                        tcb_relation_def
+                 split: Structures_A.kernel_object.split_asm if_split_asm
+                        arch_kernel_obj.split_asm)+
+  apply fastforce
+  done
+
+lemma st_tcb_at_coerce_concrete:
+  assumes t: "st_tcb_at P t s"
+  assumes sr: "(s, s') \<in> state_relation" "pspace_aligned s" "pspace_distinct s"
+  shows "st_tcb_at' (\<lambda>st'. \<exists>st. thread_state_relation st st' \<and> P st) t s'"
+  using assms
+  apply (clarsimp simp: state_relation_def pred_tcb_at_def obj_at_def projectKOs)
+  apply (frule (1) pspace_distinct_cross, fastforce simp: state_relation_def)
+  apply (frule pspace_aligned_cross, fastforce simp: state_relation_def)
+  apply (prop_tac "tcb_at t s", clarsimp simp: st_tcb_at_def obj_at_def is_tcb)
+  apply (drule (2) tcb_at_cross[rotated], fastforce simp: state_relation_def)
+  apply (clarsimp simp: state_relation_def pred_tcb_at'_def obj_at'_def projectKOs)
+  apply (erule (1) pspace_dom_relatedE)
+  apply (erule (1) obj_relation_cutsE, simp_all)
+   apply (clarsimp simp: st_tcb_at'_def obj_at'_def other_obj_relation_def tcb_relation_def
+                  split: Structures_A.kernel_object.split_asm if_split_asm)+
+  apply fastforce
+  done
+
+lemma st_tcb_at_runnable_cross:
+  "\<lbrakk> st_tcb_at runnable t s; pspace_aligned s; pspace_distinct s; (s, s') \<in> state_relation \<rbrakk>
+       \<Longrightarrow> st_tcb_at' runnable' t s'"
+  apply (drule (3) st_tcb_at_coerce_concrete)
+  by (clarsimp simp: pred_tcb_at'_def obj_at'_def sts_rel_runnable)
+
+lemma bound_sc_tcb_at_cross:
+  assumes t: "bound_sc_tcb_at P t s"
+  assumes sr: "(s, s') \<in> state_relation" "pspace_aligned s" "pspace_distinct s"
+  shows "tcb_at' t s' \<and> P (tcbSCs_of s' t)"
+  using assms
+  apply (clarsimp simp: state_relation_def pred_tcb_at_def obj_at_def projectKOs)
+  apply (frule (1) pspace_distinct_cross, fastforce simp: state_relation_def)
+  apply (frule pspace_aligned_cross, fastforce simp: state_relation_def)
+  apply (prop_tac "tcb_at t s", clarsimp simp: obj_at_def is_tcb)
+  apply (drule (2) tcb_at_cross[rotated], fastforce simp: state_relation_def)
+  apply (clarsimp simp: state_relation_def pred_tcb_at'_def obj_at'_def projectKOs opt_map_red)
+  apply (erule (1) pspace_dom_relatedE)
+  apply (erule (1) obj_relation_cutsE, simp_all)
+   apply (clarsimp simp: st_tcb_at'_def obj_at'_def other_obj_relation_def tcb_relation_def
+                  split: Structures_A.kernel_object.split_asm if_split_asm)+
+  done
+
+lemma bound_yt_tcb_at_cross:
+  assumes t: "bound_yt_tcb_at P t s"
+  assumes sr: "(s, s') \<in> state_relation" "pspace_aligned s" "pspace_distinct s"
+  shows "obj_at' (\<lambda>tcb'. \<exists>tcb. tcb_relation tcb tcb' \<and> P (tcb_yield_to tcb)) t s'"
+  using assms
+  apply (clarsimp simp: state_relation_def pred_tcb_at_def obj_at_def projectKOs)
+  apply (frule (1) pspace_distinct_cross, fastforce simp: state_relation_def)
+  apply (frule pspace_aligned_cross, fastforce simp: state_relation_def)
+  apply (prop_tac "tcb_at t s", clarsimp simp: st_tcb_at_def obj_at_def is_tcb)
+  apply (drule (2) tcb_at_cross[rotated], fastforce simp: state_relation_def)
+  apply (clarsimp simp: state_relation_def pred_tcb_at'_def obj_at'_def projectKOs)
+  apply (erule (1) pspace_dom_relatedE)
+  apply (erule (1) obj_relation_cutsE, simp_all)
+   apply (clarsimp simp: st_tcb_at'_def obj_at'_def other_obj_relation_def tcb_relation_def
+                  split: Structures_A.kernel_object.split_asm if_split_asm)+
+  apply fastforce
+  done
+
+lemma sc_tcb_sc_at_bound_cross:
+  "\<lbrakk>pspace_relation (kheap s) (ksPSpace s'); valid_objs s; pspace_aligned s; pspace_distinct s;
+    sc_tcb_sc_at ((\<noteq>) None) scp s\<rbrakk>
+  \<Longrightarrow> obj_at' (\<lambda>sc. \<exists>y. scTCB sc = Some y) scp s'"
+  apply (clarsimp simp: obj_at_def sc_tcb_sc_at_def)
+  apply (frule (1) pspace_relation_absD)
+  apply clarsimp
+  apply (prop_tac "valid_sched_context_size n")
+   apply (erule (1) valid_sched_context_size_objsI)
+  apply (clarsimp simp: if_split_asm)
+  apply (rename_tac z; case_tac z; simp)
+  apply (drule (3) aligned_distinct_ko_at'I[where 'a=sched_context], simp)
+  apply (clarsimp simp: obj_at'_def sc_relation_def projectKOs)
+  by (metis not_None_eq)
+
+lemma cur_tcb_cross:
+  "\<lbrakk> cur_tcb s; pspace_aligned s; pspace_distinct s; (s,s') \<in> state_relation \<rbrakk> \<Longrightarrow> cur_tcb' s'"
+  apply (clarsimp simp: cur_tcb'_def cur_tcb_def state_relation_def)
+  apply (erule (3) tcb_at_cross)
+  done
+
+method add_cur_tcb' =
+  rule_tac Q="\<lambda>s'. cur_tcb' s'" in corres_cross_add_guard,
+  fastforce intro!: cur_tcb_cross
+
+lemma cur_sc_tcb_cross:
+  "\<lbrakk>(s, s') \<in> state_relation; valid_objs s; pspace_aligned s; pspace_distinct s;
+    cur_sc_tcb s; schact_is_rct s\<rbrakk>
+  \<Longrightarrow> obj_at' (\<lambda>sc. scTCB sc = Some (ksCurThread s')) (ksCurSc s') s'"
+  apply (clarsimp simp: obj_at_def sc_tcb_sc_at_def cur_sc_tcb_def
+                 dest!: schact_is_rct state_relationD)
+  apply (frule (1) pspace_relation_absD)
+  apply clarsimp
+  apply (prop_tac "valid_sched_context_size n")
+   apply (erule (1) valid_sched_context_size_objsI)
+  apply (clarsimp simp: if_split_asm)
+  apply (rename_tac z; case_tac z; simp)
+  apply (drule (3) aligned_distinct_ko_at'I[where 'a=sched_context], simp)
+  apply (clarsimp simp: obj_at'_def sc_relation_def projectKOs)
+  done
+
+lemma reply_at_cross:
+  assumes p: "pspace_relation (kheap s) (ksPSpace s')"
+  assumes ps: "pspace_aligned s" "pspace_distinct s"
+  assumes t: "reply_at ptr s"
+  shows "reply_at' ptr s'"
+  using assms
+  apply (clarsimp simp: obj_at_def is_reply)
+  apply (drule (1) pspace_relation_absD, clarsimp)
+  apply (case_tac z; simp)
+  by (fastforce dest!: aligned_distinct_ko_at'I[where 'a=reply] elim: obj_at'_weakenE)
+
+lemma ep_at_cross:
+  assumes p: "pspace_relation (kheap s) (ksPSpace s')"
+  assumes ps: "pspace_aligned s" "pspace_distinct s"
+  assumes t: "ep_at ptr s"
+  shows "ep_at' ptr s'"
+  using assms
+  apply (clarsimp simp: obj_at_def is_ep)
+  apply (drule (1) pspace_relation_absD, clarsimp simp: other_obj_relation_def)
+  apply (case_tac z; simp)
+  by (fastforce dest!: aligned_distinct_ko_at'I[where 'a=endpoint] elim: obj_at'_weakenE)
+
+lemma ntfn_at_cross:
+  assumes p: "pspace_relation (kheap s) (ksPSpace s')"
+  assumes ps: "pspace_aligned s" "pspace_distinct s"
+  assumes t: "ntfn_at ptr s"
+  shows "ntfn_at' ptr s'"
+  using assms
+  apply (clarsimp simp: obj_at_def is_ntfn)
+  apply (drule (1) pspace_relation_absD, clarsimp simp: other_obj_relation_def)
+  apply (case_tac z; simp)
+  by (fastforce dest!: aligned_distinct_ko_at'I[where 'a=notification] elim: obj_at'_weakenE)
+
+lemma sc_at_cross:
+  assumes p: "pspace_relation (kheap s) (ksPSpace s')"
+  assumes ps: "pspace_aligned s" "pspace_distinct s"
+  assumes t: "sc_at ptr s"
+  shows "sc_at' ptr s'"
+  using assms
+  apply (clarsimp simp: obj_at_def is_sc_obj)
+  apply (drule (1) pspace_relation_absD, clarsimp)
+  apply (case_tac z; simp)
+  by (fastforce dest!: aligned_distinct_ko_at'I[where 'a=sched_context] elim: obj_at'_weakenE)
+
+lemma sc_at'_cross_rel:
+  "cross_rel (pspace_aligned and pspace_distinct and sc_at t) (sc_at' t)"
+  unfolding cross_rel_def state_relation_def
+  apply clarsimp
+  by (erule (3) sc_at_cross)
+
+lemma sc_obj_at_cross:
+  assumes p: "pspace_relation (kheap s) (ksPSpace s')"
+  assumes ps: "pspace_aligned s" "pspace_distinct s"
+  assumes t: "sc_obj_at n ptr s"
+  shows "obj_at' (\<lambda>sc::sched_context. objBits sc = minSchedContextBits + n) ptr s'"
+  using assms
+  apply (clarsimp simp: obj_at_def is_sc_obj)
+  apply (drule (1) pspace_relation_absD, clarsimp)
+  apply (case_tac z; simp)
+  apply (rename_tac sc')
+  apply (drule (3) aligned_distinct_ko_at'I[where 'a=sched_context], simp)
+  by (clarsimp simp: scBits_simps objBits_simps sc_relation_def obj_at'_def)
+
+lemma real_cte_at_cross:
+  assumes p: "pspace_relation (kheap s) (ksPSpace s')"
+  assumes ps: "pspace_aligned s" "pspace_distinct s"
+  assumes t: "real_cte_at ptr s"
+  shows "real_cte_at' (cte_map ptr) s'"
+  using assms
+  apply (clarsimp simp: obj_at_def is_ntfn)
+  apply (drule (1) pspace_relation_absD)
+  apply (clarsimp simp: is_cap_table other_obj_relation_def well_formed_cnode_n_def)
+  apply (prop_tac "\<exists>z. ksPSpace s' (cte_map (fst ptr, snd ptr)) = Some z \<and>
+    cte_relation (snd ptr) (CNode (length (snd ptr)) cs) z")
+  apply fastforce
+  apply (clarsimp split: kernel_object.split_asm simp: cte_relation_def)
+  by (fastforce dest!: aligned_distinct_ko_at'I[where 'a=cte] elim: obj_at'_weakenE)
+
+lemma valid_tcb_state_cross:
+  assumes "pspace_relation (kheap s) (ksPSpace s')"
+          "thread_state_relation ts ts'"
+          "pspace_aligned s"
+          "pspace_distinct s"
+          "valid_tcb_state ts s"
+  shows "valid_tcb_state' ts' s'" using assms
+  by (fastforce dest: ep_at_cross reply_at_cross ntfn_at_cross
+                simp: valid_bound_obj'_def valid_tcb_state_def valid_tcb_state'_def
+               split: Structures_A.thread_state.split_asm option.split_asm)
+
+lemma state_refs_of_cross_eq:
+  "\<lbrakk>(s, s') \<in> state_relation; pspace_aligned s; pspace_distinct s\<rbrakk>
+       \<Longrightarrow> state_refs_of' s' = state_refs_of s"
+  apply (rule sym)
+  apply (rule ext, rename_tac p)
+  apply (frule state_relation_pspace_relation)
+  apply (frule (2) pspace_distinct_cross)
+  apply (frule (1) pspace_aligned_cross)
+  apply (clarsimp simp: state_refs_of_def state_refs_of'_def
+                 split: option.split)
+  apply (rule conjI; clarsimp)
+   apply (rename_tac ko')
+   apply (erule (1) pspace_dom_relatedE)
+   apply (rename_tac ko P; case_tac ko; clarsimp split: if_split_asm simp: cte_relation_def)
+   apply (rename_tac ako; case_tac ako; clarsimp simp: pte_relation_def)
+  apply (rule conjI; clarsimp)
+   apply (drule (1) pspace_relation_None; clarsimp)
+  apply (rule conjI[rotated]; clarsimp)
+   apply (frule pspace_relation_pspace_bounded'[OF state_relation_pspace_relation])
+   apply (frule pspace_alignedD'; frule pspace_boundedD'; clarsimp dest!: pspace_distinctD')
+  apply (rename_tac ko ko')
+  apply (frule (1) pspace_relation_absD)
+  apply (case_tac ko; clarsimp split: if_split_asm)
+        apply (rename_tac n sz, drule_tac x=p and y="cte_relation (replicate n False)" in spec2)
+        apply (fastforce simp: cte_relation_def cte_map_def well_formed_cnode_n_def)
+       apply (find_goal \<open>match premises in "_ = Some (ArchObj _)" \<Rightarrow> -\<close>)
+       apply (rename_tac ako; case_tac ako; simp)
+          apply (case_tac ko'; clarsimp simp: other_obj_relation_def)
+         apply ((drule_tac x=0 in spec, clarsimp simp:  pte_relation_def)+)[1]
+       apply (drule_tac x=p in spec)
+       apply (rename_tac b sz)
+       apply (drule_tac x="\<lambda>_ obj. obj = (if b then KOUserDataDevice else KOUserData)" in spec, clarsimp)
+       apply (simp only: imp_ex)
+       apply (drule_tac x=0 in spec, clarsimp simp: pageBitsForSize_def ptTranslationBits_def
+                                             split: vmpage_size.split_asm)
+      apply (all \<open>case_tac ko'; clarsimp simp: other_obj_relation_def\<close>)
+      apply (rename_tac tcb tcb';
+             clarsimp simp: tcb_relation_def arch_tcb_relation_def fault_rel_optionation_def
+                            thread_state_relation_def tcb_st_refs_of_def tcb_st_refs_of'_def;
+             rename_tac tcb'; case_tac "tcb_state tcb"; case_tac "tcbState tcb'";
+             clarsimp simp: tcb_bound_refs'_def get_refs_def2 split: option.splits)
+     apply (clarsimp simp: ep_q_refs_of_def ep_relation_def split: Structures_A.endpoint.splits)
+    apply (clarsimp simp: ntfn_q_refs_of_def ntfn_relation_def split: Structures_A.ntfn.splits)
+   apply (clarsimp simp: sc_relation_def get_refs_def2)
+   apply (drule state_relation_sc_replies_relation)
+   apply (frule sc_replies_relation_scReplies_of)
+     apply (fastforce simp: obj_at_def is_sc_obj_def)
+    apply (clarsimp simp: opt_map_def)
+   apply (clarsimp simp: opt_map_def sc_replies_of_scs_def map_project_def scs_of_kh_def)
+  apply (clarsimp simp: reply_relation_def split: Structures_A.ntfn.splits)
+  done
+
+end
+
+lemma state_refs_of_cross:
+  "\<lbrakk>P (state_refs_of s); (s, s') \<in> state_relation; pspace_aligned s; pspace_distinct s\<rbrakk>
+      \<Longrightarrow> P (state_refs_of' s')"
+  by (clarsimp simp: state_refs_of_cross_eq elim!: rsubst[where P=P])
+
+lemma ct_not_inQ_cross:
+  "\<lbrakk>(s,s') \<in> state_relation; ct_not_in_q s; valid_queues' s'; cur_tcb s; pspace_aligned s;
+    pspace_distinct s\<rbrakk>
+   \<Longrightarrow> ct_not_inQ s'"
+  apply (frule (3) cur_tcb_cross)
+  apply (clarsimp simp: ct_not_inQ_def ct_not_in_q_def)
+  apply (prop_tac "scheduler_action s = resume_cur_thread")
+   apply (clarsimp simp: state_relation_def)
+   apply (metis sched_act_relation.simps Structures_A.scheduler_action.exhaust
+                scheduler_action.simps)
+  apply (clarsimp simp: not_queued_def)
+  apply (rule ccontr)
+  apply (prop_tac "obj_at' tcbQueued (ksCurThread s') s'")
+   apply (clarsimp simp: obj_at_simps cur_tcb'_def)
+  apply (frule curthread_relation)
+  apply (frule state_relation_ready_queues_relation)
+  apply (clarsimp simp: valid_queues'_def inQ_def ready_queues_relation_def obj_at_simps)
+  by (metis Structures_H.kernel_object.case(6))
+
+lemma sch_act_wf_cross:
+  "\<lbrakk>(s,s') \<in> state_relation; valid_sched_action s; cur_tcb s; pspace_aligned s; pspace_distinct s\<rbrakk>
+   \<Longrightarrow> sch_act_wf (ksSchedulerAction s') s'"
+  apply (clarsimp simp: sch_act_wf_def)
+  apply (cases "ksSchedulerAction s'"; clarsimp)
+   apply (prop_tac "scheduler_action s = resume_cur_thread")
+    apply (clarsimp simp: state_relation_def)
+    apply (metis sched_act_relation.simps Structures_A.scheduler_action.exhaust
+                 scheduler_action.simps)
+   apply (frule curthread_relation)
+   apply (frule state_relation_pspace_relation)
+   apply (frule (2) cur_tcb_cross)
+    apply fastforce
+   apply (clarsimp simp: valid_sched_action_def is_activatable_def vs_all_heap_simps
+                         ct_in_state'_def st_tcb_at'_def)
+   apply (clarsimp simp: pspace_relation_def)
+   apply (drule_tac x="cur_thread s" in bspec, fastforce)
+   apply (drule_tac x="(cur_thread s, other_obj_relation)" in bspec, fastforce)
+   apply (clarsimp simp: other_obj_relation_def)
+   apply (rename_tac tcb)
+   apply (case_tac "tcb_state tcb"; clarsimp simp: tcb_relation_def obj_at_simps cur_tcb'_def)
+  apply (rename_tac target)
+  apply (clarsimp simp: valid_sched_action_def weak_valid_sched_action_def vs_all_heap_simps)
+  apply (prop_tac "scheduler_action s = switch_thread target")
+   apply (clarsimp simp: state_relation_def)
+   apply (metis sched_act_relation.simps Structures_A.scheduler_action.exhaust
+                scheduler_action.simps)
+  apply (prop_tac "tcb_at' target s'")
+   apply (fastforce intro!: tcb_at_cross
+                      simp: obj_at_def is_tcb_def)
+  apply (frule state_relation_pspace_relation)
+  apply (clarsimp simp: pspace_relation_def)
+  apply (drule_tac x=target in bspec, fastforce)
+  apply (drule_tac x="(target, other_obj_relation)" in bspec, fastforce)
+  apply (clarsimp simp: other_obj_relation_def)
+  apply (intro conjI)
+   apply (fastforce intro!: st_tcb_at_runnable_cross
+                      simp: obj_at_def pred_tcb_at_def)
+  apply (clarsimp simp: tcb_relation_def obj_at_simps switch_in_cur_domain_def
+                        state_relation_def in_cur_domain_def tcb_in_cur_domain'_def
+                        etcb_at'_def vs_all_heap_simps)
+  done
+
+lemma ct_idle_or_in_cur_domain'_cross:
+  "\<lbrakk>(s,s') \<in> state_relation; ct_in_cur_domain s; cur_tcb s; pspace_aligned s; pspace_distinct s\<rbrakk>
+   \<Longrightarrow> ct_idle_or_in_cur_domain' s'"
+  apply (clarsimp simp: ct_idle_or_in_cur_domain'_def tcb_in_cur_domain'_def ct_in_cur_domain_def)
+  apply (case_tac "cur_thread s = idle_thread s"; clarsimp)
+   apply (clarsimp simp: state_relation_def)
+  apply (frule curthread_relation)
+  apply (frule (2) cur_tcb_cross)
+   apply fastforce
+  apply (prop_tac "scheduler_action s = resume_cur_thread")
+   apply (clarsimp simp: state_relation_def)
+   apply (metis sched_act_relation.simps Structures_A.scheduler_action.exhaust
+                scheduler_action.simps)
+  apply (clarsimp simp: in_cur_domain_def etcb_at_def vs_all_heap_simps obj_at_simps cur_tcb'_def)
+  apply (frule state_relation_pspace_relation)
+  apply (clarsimp simp: pspace_relation_def)
+  apply (drule_tac x="cur_thread s" in bspec)
+   apply (clarsimp simp: cur_tcb_def obj_at_def)
+  apply (drule_tac x="(cur_thread s, other_obj_relation)" in bspec)
+   apply (clarsimp simp: cur_tcb_def obj_at_def is_tcb_def)
+   apply (rename_tac tcb)
+   apply (case_tac tcb; clarsimp)
+  apply (clarsimp simp: cur_tcb_def obj_at_def is_tcb_def)
+  apply (rename_tac tcb)
+  apply (case_tac tcb; clarsimp)
+  apply (clarsimp simp: other_obj_relation_def tcb_relation_def state_relation_def)
+  done
+
+lemma valid_idle'_cross:
+  "\<lbrakk>(s,s') \<in> state_relation; valid_idle s; pspace_aligned s; pspace_distinct s; valid_objs s\<rbrakk>
+   \<Longrightarrow> valid_idle' s'"
+  apply (clarsimp simp: valid_idle'_def valid_idle_def pred_tcb_at_def obj_at_def)
+  apply (prop_tac "ksIdleThread s' = idle_thread s")
+   apply (clarsimp simp: state_relation_def)
+  apply clarsimp
+  apply (prop_tac "tcb_at' (ksIdleThread s') s'")
+   apply (fastforce intro!: tcb_at_cross simp: obj_at_def state_relation_def is_tcb_def)
+  apply (prop_tac "sc_at' (idle_sc_ptr) s'")
+   apply (fastforce intro!: sc_at_cross valid_objs_valid_sched_context_size
+                      simp: obj_at_def state_relation_def is_sc_obj_def)
+  apply (frule state_relation_pspace_relation)
+  apply (clarsimp simp: pspace_relation_def)
+  apply (intro conjI)
+   apply (drule_tac x="idle_thread s" in bspec, fastforce)
+   apply (drule_tac x="(idle_thread s, other_obj_relation)" in bspec, fastforce)
+   apply (clarsimp simp: obj_at_simps idle_tcb'_def tcb_relation_def)
+  apply (drule_tac x="idle_sc_ptr" in bspec, fastforce)
+  apply (drule_tac x="(idle_sc_ptr, sc_relation_cut)" in bspec)
+   apply (fastforce intro: valid_objs_valid_sched_context_size)
+  by (fastforce dest: sc_replies_prevs_walk
+                simp: heap_walk_Nil_None obj_at_simps sc_relation_def state_relation_def)
+
+lemma ksReadyQueues_distinct_cross:
+   "\<lbrakk>(s,s') \<in> state_relation; valid_ready_qs s\<rbrakk> \<Longrightarrow> \<forall>d p. distinct (ksReadyQueues s' (d, p))"
+   by (clarsimp simp: valid_ready_qs_def state_relation_def ready_queues_relation_def)
+
+lemma ready_qs_runnable_cross:
+  "\<lbrakk>(s, s') \<in> state_relation; pspace_aligned s; pspace_distinct s; valid_ready_qs s\<rbrakk>
+   \<Longrightarrow> ready_qs_runnable s'"
+  unfolding ready_qs_runnable_def
+  by (fastforce simp: state_relation_def ready_queues_relation_def
+                      in_ready_q_def st_tcb_at_runnable_cross
+                dest: valid_ready_qs_in_ready_qD)
+
+lemma replyTCBs_of_cross:
+  "\<lbrakk>(s, s') \<in> state_relation; reply_tcb_reply_at P rptr s\<rbrakk>
+   \<Longrightarrow> P (replyTCBs_of s' rptr)"
+  apply (clarsimp simp: reply_at_ppred_def obj_at_def state_relation_def)
+  apply (drule (1) pspace_relation_absD, clarsimp simp: other_obj_relation_def)
+  apply (case_tac z; simp)
+  apply (clarsimp simp: opt_map_def reply_relation_def)
+  done
+
+lemma replySCs_of_cross:
+  "\<lbrakk>(s, s') \<in> state_relation; reply_sc_reply_at P rptr s\<rbrakk>
+   \<Longrightarrow> P (replySCs_of s' rptr)"
+  apply (clarsimp simp: reply_at_ppred_def obj_at_def is_tcb state_relation_def)
+  apply (drule (1) pspace_relation_absD, clarsimp simp: other_obj_relation_def)
+  apply (case_tac z; simp)
+  apply (clarsimp simp: opt_map_def reply_relation_def)
+  done
+
+lemma valid_replies_sc_cross:
+  "\<lbrakk>(s, s') \<in> state_relation; valid_replies s; sym_refs (state_refs_of s);
+    pspace_aligned s; pspace_distinct s; reply_at rptr s\<rbrakk>
+   \<Longrightarrow> valid_replies'_sc_asrt rptr s'"
+  apply (clarsimp simp: valid_replies_defs valid_replies'_sc_asrt_def)
+  apply (rename_tac scptr rp ko)
+  apply (prop_tac "sc_replies_sc_at (\<lambda>rs. rptr \<in> set rs) scptr s")
+   apply (frule_tac sc_ptr=scptr and reply_ptr=rptr in sym_refs_sc_replies_sc_at)
+    apply (rule ccontr)
+    apply (drule not_sk_obj_at_pred)
+     apply (fastforce simp: sk_obj_at_pred_def obj_at_def is_obj_defs)
+    apply (frule (1) replySCs_of_cross)
+    apply (clarsimp simp: obj_at'_def projectKOs opt_map_def)
+   apply (clarsimp simp: sc_at_pred_n_eq_commute sc_at_ppred_def obj_at_def)
+  apply (drule subsetD, force)
+  apply (clarsimp simp: pred_tcb_at_eq_commute[symmetric])
+  apply (frule (1) st_tcb_reply_state_refs)
+  apply (drule (3) st_tcb_at_coerce_concrete)
+  apply (drule replyTCBs_of_cross[where P="\<lambda>rtcb. rtcb = (Some tptr)" for tptr])
+   apply (fastforce simp: sk_obj_at_pred_def2)
+  apply (clarsimp simp: pred_tcb_at'_def obj_at'_def)
+  done
+
+lemma getCurThread_sp:
+  "\<lbrace>P\<rbrace> getCurThread \<lbrace>\<lambda>rv. P and (\<lambda>s. rv = ksCurThread s)\<rbrace>"
+  by (wpsimp simp: getCurThread_def)
+
+lemma getSchedulerAction_sp:
+  "\<lbrace>P\<rbrace> getSchedulerAction \<lbrace>\<lambda>rv. P and (\<lambda>s. rv = ksSchedulerAction s)\<rbrace>"
+  by (wpsimp simp: getSchedulerAction_def)
+
+lemma getReprogramTimer_sp:
+  "\<lbrace>P\<rbrace> getReprogramTimer \<lbrace>\<lambda>rv. P and (\<lambda>s. rv = ksReprogramTimer s)\<rbrace>"
+  by (wpsimp simp: getReprogramTimer_def)
+
+lemma getIdleThread_sp:
+  "\<lbrace>P\<rbrace> getIdleThread \<lbrace>\<lambda>rv. P and (\<lambda>s. rv = ksIdleThread s)\<rbrace>"
+  by wpsimp
+
+lemma getIdleSC_sp:
+  "\<lbrace>P\<rbrace> getIdleSC \<lbrace>\<lambda>rv. P and (\<lambda>s. rv = ksIdleSC s)\<rbrace>"
+  by wpsimp
+
+lemma getReprogramTimer_wp[wp]:
+  "\<lbrace>\<lambda>s. P (ksReprogramTimer s) s\<rbrace> getReprogramTimer \<lbrace>P\<rbrace>"
+  by (wpsimp simp: getReprogramTimer_def)
+
+lemma getConsumedTime_wp[wp]:
+  "\<lbrace>\<lambda>s. P (ksConsumedTime s) s\<rbrace> getConsumedTime \<lbrace>P\<rbrace>"
+  by (wpsimp simp: getConsumedTime_def)
+
+lemma isRoundRobin_wp:
+  "\<lbrace>\<lambda>s. \<forall>ko. ko_at' ko sc s \<longrightarrow> P (scPeriod ko = 0) s\<rbrace> isRoundRobin sc \<lbrace>P\<rbrace>"
+  by (wpsimp simp: isRoundRobin_def)
+
+lemma getCurSc_wp[wp]:
+  "\<lbrace>\<lambda>s. P (ksCurSc s) s\<rbrace> getCurSc \<lbrace>P\<rbrace>"
+  unfolding getCurSc_def
+  by wpsimp
+
+lemma getCurTime_wp[wp]:
+  "\<lbrace>\<lambda>s. P (ksCurTime s) s\<rbrace> getCurTime \<lbrace>P\<rbrace>"
+  unfolding getCurTime_def
+  by wpsimp
+
+lemma curDomain_wp[wp]:
+  "\<lbrace>\<lambda>s. P (ksCurDomain s) s\<rbrace> curDomain \<lbrace>P\<rbrace>"
+  unfolding curDomain_def
+  by wpsimp
+
+lemma curDomain_sp:
+  "\<lbrace>P\<rbrace> curDomain \<lbrace>\<lambda>rv. P and (\<lambda>s. rv = ksCurDomain s)\<rbrace>"
+  by wpsimp
+
+lemma getReleaseQueue_wp[wp]:
+  "\<lbrace>\<lambda>s. P (ksReleaseQueue s) s\<rbrace> getReleaseQueue \<lbrace>P\<rbrace>"
+  unfolding getReleaseQueue_def
+  by wpsimp
+
+lemma getObject_sc_wp:
+  "\<lbrace>\<lambda>s. sc_at' p s \<longrightarrow> (\<exists>t::sched_context. ko_at' t p s \<and> Q t s)\<rbrace> getObject p \<lbrace>Q\<rbrace>"
+  by (clarsimp simp: getObject_def valid_def in_monad
+                     split_def objBits_simps' loadObject_default_def
+                     projectKOs obj_at'_def in_magnitude_check
+              dest!: readObject_misc_ko_at')
+
+lemma getRefillNext_getSchedContext:
+  "getRefillNext scPtr index = do sc \<leftarrow> getSchedContext scPtr;
+                                  return $ if index = scRefillMax sc - 1 then 0 else index + 1
+                               od"
+  apply (clarsimp simp: getRefillNext_def readRefillNext_def readSchedContext_def
+                        getSchedContext_def getObject_def[symmetric])
+  done
+
+lemma getRefillNext_wp:
+  "\<lbrace>\<lambda>s. \<forall>ko. ko_at' ko scPtr s \<longrightarrow> P (if index = scRefillMax ko - Suc 0 then 0 else index + 1) s\<rbrace>
+   getRefillNext scPtr index
+   \<lbrace>P\<rbrace>"
+  apply (simp add: getRefillNext_getSchedContext)
+  apply (wpsimp wp: getObject_sc_wp)
+  done
+
+lemma getRefillSize_def2:
+  "getRefillSize scPtr = liftM scRefillCount (gets_the (readSchedContext scPtr))"
+  apply (clarsimp simp: getRefillSize_def readRefillSize_def liftM_def oliftM_def)
+  done
+
+lemma getRefillSize_wp:
+  "\<lbrace>\<lambda>s. \<forall>ko. ko_at' ko scp s \<longrightarrow> P (scRefillCount ko) s\<rbrace> getRefillSize scp \<lbrace>P\<rbrace>"
+  apply (clarsimp simp: getRefillSize_def2)
+  apply (wpsimp wp: simp: readSchedContext_def)
+  done
+
+lemma refillEmpty_wp:
+  "\<lbrace>\<lambda>s. \<forall>ko. ko_at' ko scp s \<longrightarrow> P (scRefillCount ko = 0) s\<rbrace> refillEmpty scp \<lbrace>P\<rbrace>"
+  unfolding refillEmpty_def
+  by (wpsimp wp:)
+
+lemma refillFull_wp:
+  "\<lbrace>\<lambda>s. \<forall>ko. ko_at' ko scp s \<longrightarrow> P (scRefillCount ko = scRefillMax ko) s\<rbrace> refillFull scp \<lbrace>P\<rbrace>"
+  unfolding refillFull_def
+  by (wpsimp wp:)
+
+lemma no_ofail_readCurTime[simp]:
+  "no_ofail \<top> readCurTime"
+  unfolding readCurTime_def by clarsimp
+
+lemma ovalid_readCurTime[wp]:
+  "o\<lbrace>\<lambda>s. P (ksCurTime s) s\<rbrace> readCurTime \<lbrace>\<lambda>r s. P r s \<and> r = ksCurTime s\<rbrace>"
+  by (simp add: readCurTime_def asks_def obind_def ovalid_def)
+
+lemma ovalid_readRefillReady[rule_format, simp]:
+  "ovalid (\<lambda>s. \<forall>ko. ko_at' ko scp s \<longrightarrow> P (rTime (refillHd ko) \<le> ksCurTime s + kernelWCETTicks) s)
+              (readRefillReady scp) P"
+  unfolding readRefillReady_def readSchedContext_def ovalid_def
+  by (fastforce simp: obind_def split: option.split_asm
+                dest: use_ovalid[OF ovalid_readCurTime]
+               dest!: readObject_misc_ko_at')
+
+
+lemma refillReady_wp:
+  "\<lbrace>\<lambda>s. \<forall>ko. ko_at' ko scp s \<longrightarrow> P (rTime (refillHd ko) \<le> ksCurTime s + kernelWCETTicks) s\<rbrace> refillReady scp \<lbrace>P\<rbrace>"
+  unfolding refillReady_def
+  by wpsimp (drule use_ovalid[OF ovalid_readRefillReady])
+
+lemma scActive_wp:
+  "\<lbrace>\<lambda>s. \<forall>ko. ko_at' ko scp s \<longrightarrow> P (0 < scRefillMax ko) s\<rbrace> scActive scp \<lbrace>P\<rbrace>"
+  unfolding scActive_def
+  by wpsimp
+
+lemma getRefills_wp:
+  "\<lbrace>\<lambda>s. \<forall>ko. ko_at' ko scp s \<longrightarrow> P (scRefills ko) s\<rbrace>
+   getRefills scp
+   \<lbrace>P\<rbrace>"
+  unfolding getRefills_def
+  by wpsimp
+
+lemma refillSufficient_wp:
+  "\<lbrace>\<lambda>s. \<forall>ko. ko_at' ko scp s \<longrightarrow> P (minBudget \<le> refillsCapacity k (scRefills ko) (scRefillHead ko)) s\<rbrace> refillSufficient scp k \<lbrace>P\<rbrace>"
+  unfolding refillSufficient_def
+  apply (wpsimp wp: getRefills_wp)
+  by (clarsimp simp: sufficientRefills_def obj_at'_def)
+
+(* projection rewrites *)
+
+lemma pred_map_rewrite:
+  "pred_map P proj = opt_pred P proj"
+  by (fastforce simp: pred_map_def2)
+
+abbreviation sc_of2 :: "Structures_A.kernel_object \<rightharpoonup> Structures_A.sched_context" where
+  "sc_of2 ko \<equiv> case ko of kernel_object.SchedContext sc n \<Rightarrow> Some sc | _ \<Rightarrow> None"
+
+abbreviation scs_of2 :: "'z state \<Rightarrow> obj_ref \<rightharpoonup> Structures_A.sched_context" where
+  "scs_of2 \<equiv> (\<lambda>s. kheap s |> sc_of2)"
+
+lemma scs_of_rewrite:
+  "scs_of s = scs_of2 s"
+  by (fastforce simp: sc_heap_of_state_def opt_map_def
+              split: option.splits Structures_A.kernel_object.splits)
+
+abbreviation
+  "sc_replies_of2 s \<equiv> scs_of2 s ||> sc_replies"
+
+lemma sc_replies_of_rewrite:
+  "sc_replies_of s = sc_replies_of2 s"
+  by (fastforce simp: sc_heap_of_state_def sc_replies_of_scs_def opt_map_def map_project_def
+              split: option.splits Structures_A.kernel_object.splits)
+
+definition
+  sc_replies_relation2_2 ::
+  "(obj_ref \<rightharpoonup> obj_ref list) \<Rightarrow> (obj_ref \<rightharpoonup> obj_ref) \<Rightarrow> (obj_ref \<rightharpoonup> obj_ref) \<Rightarrow> bool" where
+  "sc_replies_relation2_2 sc_repls scRepl replPrevs \<equiv>
+     \<forall>p replies. sc_repls p = Some replies \<longrightarrow> heap_ls replPrevs (scRepl p) replies"
+
+abbreviation sc_replies_relation2 :: "det_state \<Rightarrow> kernel_state \<Rightarrow> bool" where
+  "sc_replies_relation2 s s' \<equiv>
+    sc_replies_relation2_2 (sc_replies_of2 s) (scReplies_of s') (replyPrevs_of s')"
+
+lemmas sc_replies_relation2_def = sc_replies_relation2_2_def
+
+lemma sc_replies_relation_rewrite:
+  "sc_replies_relation s s' = sc_replies_relation2 s s'"
+  unfolding sc_replies_relation_def sc_replies_relation2_def sc_replies_of_rewrite
+  by simp
+
+definition is_active_sc2 where
+  "is_active_sc2 p s \<equiv> ((\<lambda>sc. 0 < sc_refill_max sc) |< scs_of2 s) p"
+
+lemma is_active_sc_rewrite:
+  "is_active_sc p s = is_active_sc2 p s"
+  by (fastforce simp: is_active_sc2_def vs_all_heap_simps is_active_sc_def
+                      active_sc_def opt_map_red opt_map_def
+               split: option.split_asm Structures_A.kernel_object.splits)
+
+lemma active_sc_at'_imp_is_active_sc':
+  "active_sc_at' scp s \<Longrightarrow> is_active_sc' scp s"
+  by (clarsimp simp: active_sc_at'_def is_active_sc'_def obj_at'_def opt_map_def projectKOs)
+
+lemma active_sc_at'_rewrite:
+  "active_sc_at' scp s = (is_active_sc' scp s \<and> sc_at' scp s)"
+  by (fastforce simp: active_sc_at'_def is_active_sc'_def obj_at'_def opt_map_def projectKOs)
+
+abbreviation
+  "valid_refills2 scp s \<equiv>
+     ((\<lambda>sc. if sc_period sc = 0 then rr_valid_refills (sc_refills sc) (sc_refill_max sc) (sc_budget sc)
+      else sp_valid_refills (sc_refills sc) (sc_refill_max sc) (sc_period sc) (sc_budget sc)) |<
+     scs_of2 s) scp"
+
+lemmas valid_refills2_def = rr_valid_refills_def sp_valid_refills_def
+
+lemma valid_refills_rewrite:
+  "valid_refills scp s = valid_refills2 scp s"
+  by (fastforce simp: opt_map_red vs_all_heap_simps valid_refills_def
+               split: option.splits Structures_A.kernel_object.splits)
+
+definition
+  round_robin2 :: "obj_ref \<Rightarrow> 'z state \<Rightarrow> bool"
+where
+  "round_robin2 sc_ptr s \<equiv> ((\<lambda>sc. sc_period sc = 0) |< scs_of2 s) sc_ptr"
+
+lemma round_robin_rewrite:
+  "round_robin scp s = round_robin2 scp s"
+  by (clarsimp simp: round_robin_def round_robin2_def vs_all_heap_simps opt_map_def
+              split: option.splits Structures_A.kernel_object.splits)
+
+abbreviation
+  sc_refills_sc_at2 where
+  "sc_refills_sc_at2 P scp s \<equiv> ((\<lambda>sc. P (sc_refills sc)) |< scs_of2 s) scp"
+
+lemma sc_refills_sc_at_rewrite:
+  "sc_refills_sc_at P scp s = sc_refills_sc_at2 P scp s"
+  by (fastforce simp: sc_refills_sc_at_def obj_at_def is_sc_obj opt_map_red
+               split: option.splits Structures_A.kernel_object.split_asm)
+
+lemmas projection_rewrites = pred_map_rewrite scs_of_rewrite is_active_sc_rewrite
+                             sc_heap_of_state_def sc_refills_sc_at_rewrite
+                             active_sc_at'_rewrite valid_refills_rewrite round_robin_rewrite
+
+lemma is_active_sc'_cross:
+  assumes p: "pspace_relation (kheap s) (ksPSpace s')"
+  assumes t: "is_active_sc2 ptr s"
+  shows "is_active_sc' ptr s'"
+  using assms
+  supply projection_rewrites[simp]
+  apply (clarsimp simp: projectKOs is_active_sc2_def is_active_sc'_def
+                 split: option.split_asm Structures_A.kernel_object.split_asm)
+  apply (drule (1) pspace_relation_absD, clarsimp split: if_split_asm)
+  by (case_tac z; simp add: sc_relation_def opt_map_red)
+
+lemma set_refills_is_active_sc2[wp]:
+  "set_refills ptr new \<lbrace>is_active_sc2 ptr'\<rbrace>"
+  apply (wpsimp simp: is_active_sc2_def wp: set_refills_wp)
+  by (clarsimp simp: obj_at_def opt_map_def)
+
+(* end : projection rewrites *)
+
+(* updateSchedContext *)
+
+context begin interpretation Arch . (*FIXME: arch_split*)
+
+lemma state_relation_sc_update:
+  assumes
+      R1: "\<forall>s s'. (s, s') \<in> state_relation \<longrightarrow>
+         P s \<longrightarrow> P' s' \<longrightarrow> sc_at ptr s \<longrightarrow> sc_at' ptr s' \<longrightarrow>
+           (\<forall>n. (((\<lambda>ko. obj_bits ko = min_sched_context_bits + n) |< kheap s) ptr) \<longrightarrow>
+           sc_relation (the ((scs_of2 s ||> f) ptr)) n (the ((scs_of' s' ||> f') ptr)))"
+  and R2: "\<forall>s s'. (s, s') \<in> state_relation \<longrightarrow>
+         P s \<longrightarrow> P' s' \<longrightarrow> sc_at ptr s \<longrightarrow> sc_at' ptr s' \<longrightarrow>
+           heap_ls (replyPrevs_of s')  (scReply (the ((scs_of' s' ||> f') ptr)))
+             (sc_replies (the ((scs_of2 s ||> f) ptr)))"
+  and sz: "\<forall>sc'::sched_context. objBits sc' = objBits (f' sc')"
+  shows
+  "\<lbrakk>(s, s') \<in> state_relation; P s; P' s'; sc_at ptr s; sc_at' ptr s'\<rbrakk> \<Longrightarrow>
+     (kheap_update (\<lambda>hp p. if p = ptr
+                           then
+                             case hp ptr of
+                                Some (kernel_object.SchedContext sc n)
+                                   \<Rightarrow> Some (kernel_object.SchedContext (f sc) n)
+                               | _ \<Rightarrow> hp ptr
+                           else hp p) s,
+     (ksPSpace_update (\<lambda>hp' p. if p = ptr
+                               then case hp' ptr of
+                                  Some (KOSchedContext sc')
+                                     \<Rightarrow> Some (KOSchedContext (f' sc'))
+                                 | _ \<Rightarrow> hp' ptr
+                                else hp' p)) s') \<in> state_relation"
+  supply pred_map_rewrite[simp] scs_of_rewrite[simp] opt_map_red[simp]
+         sc_replies_of_rewrite[simplified, simp]
+  proof -
+  have z': "\<And>s. sc_at' ptr s
+               \<Longrightarrow> \<forall>sc'::sched_context. map_to_ctes ((\<lambda>hp' p. if p = ptr then case hp' ptr of
+                              Some (KOSchedContext sc') \<Rightarrow> Some (KOSchedContext (f' sc'))
+                            | _ \<Rightarrow> hp' ptr else hp' p) (ksPSpace s)) = map_to_ctes (ksPSpace s)"
+    by (clarsimp simp: obj_at_simps fun_upd_def[symmetric])
+  have z: "\<And>s sc'::sched_context. ko_at' sc' ptr s
+               \<Longrightarrow> map_to_ctes (ksPSpace s(ptr \<mapsto> KOSchedContext (f' sc'))) = map_to_ctes (ksPSpace s)"
+    by (clarsimp simp: obj_at_simps)
+  assume H: "(s, s') \<in> state_relation" "P s" "P' s'" "sc_at ptr s" "sc_at' ptr s'"
+  show ?thesis
+    using H sz
+    apply -
+    apply (insert R1[rule_format, OF H]
+                  R2[rule_format, OF H])
+    apply (clarsimp simp: state_relation_def)
+    apply (clarsimp simp: obj_at_def is_sc_obj)
+    apply (prop_tac "obj_at (same_caps (kernel_object.SchedContext _ n)) ptr s")
+     apply (clarsimp simp: obj_at_def obj_bits_def)
+    apply (clarsimp simp: obj_at'_def projectKOs fun_upd_def[symmetric]
+                          z[simplified obj_at'_def projectKO_eq projectKO_opts_defs])
+    apply (rename_tac n sc sc')
+    apply (rule conjI)
+     (* pspace_relation *)
+     apply (simp only: pspace_relation_def simp_thms
+                       pspace_dom_update[where x="kernel_object.SchedContext _ _"
+                                           and v="kernel_object.SchedContext _ _",
+                                         simplified a_type_def, simplified])
+     apply (simp only: dom_fun_upd2 simp_thms)
+     apply (elim conjE)
+     apply (frule bspec, erule domI)
+     apply (rule ballI, drule(1) bspec)
+     apply (drule domD)
+     apply (clarsimp simp: project_inject
+                    split: if_split_asm kernel_object.split_asm)
+     apply (drule_tac x=sc' in spec)
+     apply (rename_tac bb aa ba)
+     apply (drule_tac x="(aa, ba)" in bspec, simp)
+     apply (clarsimp simp: objBits_def)
+     apply (frule_tac ko'="kernel_object.SchedContext sc n" and x'=ptr in obj_relation_cut_same_type)
+        apply simp+
+     apply (erule obj_relation_cutsE)
+            apply ((simp split: if_split_asm)+)[8]
+    (* sc_replies_relation *)
+    apply (frule (2) sc_replies_relation_prevs_list[simplified])
+    apply (subst replyPrevs_of_non_reply_update[simplified]; (simp add: typ_at'_def ko_wp_at'_def)?)
+    apply (simp add: sc_replies_relation_def)
+    apply (rule conjI)
+     (* ghost relation *)
+     apply (clarsimp simp add: ghost_relation_def)
+     apply (erule_tac x=ptr in allE)+
+     apply (clarsimp simp: obj_at_def a_type_def is_sc_obj
+                     split: Structures_A.kernel_object.splits if_split_asm)
+    apply (rule conjI)
+     (* cdt_relation *)
+     apply (clarsimp simp add: cte_wp_at_cases cdt_relation_def)
+    (* revokable_relation *)
+    apply (prop_tac "kheap_update
+                      (\<lambda>hp x.
+                          if x = ptr
+                          then case hp ptr of None \<Rightarrow> hp ptr
+                               | Some (kernel_object.SchedContext sc n) \<Rightarrow>
+                                   Some (kernel_object.SchedContext (f sc) n)
+                               | Some _ \<Rightarrow> hp ptr
+                          else hp x) s
+             = s\<lparr> kheap := (kheap s)(ptr \<mapsto> kernel_object.SchedContext (f sc) n)\<rparr>" )
+     apply (clarsimp simp: fun_upd_def cong: if_cong)
+    apply (simp only: fun_upd_def)
+    apply (simp add: caps_of_state_after_update)
+    done
+qed
+
+(* update wp rules without ko_at' *)
+lemma updateSchedContext_wp:
+  "\<lbrace> \<lambda>s. sc_at' sc_ptr s \<longrightarrow>
+       Q (s\<lparr>ksPSpace := ksPSpace s(sc_ptr \<mapsto> KOSchedContext (f' (the (scs_of' s sc_ptr))))\<rparr>) \<rbrace>
+   updateSchedContext sc_ptr f'
+   \<lbrace> \<lambda>rv. Q \<rbrace>"
+  by (wpsimp simp: updateSchedContext_def wp: set_sc'.set_wp)
+     (clarsimp simp: obj_at'_def projectKOs opt_map_red elim!: rsubst[where P=Q])
+
+lemma no_fail_setSchedContext[wp]:
+  "no_fail (sc_at' ptr and (\<lambda>s'. ((\<lambda>k::sched_context. objBits k = objBits new) |< scs_of' s') ptr)) (setSchedContext ptr new)"
+  unfolding setSchedContext_def by (wpsimp simp: opt_map_def obj_at'_def projectKOs)
+
+lemma no_fail_updateSchedContext[wp]:
+  "no_fail (sc_at' ptr and (\<lambda>s'. ((\<lambda>k::sched_context. objBits k = objBits (f k)) |< scs_of' s') ptr))
+         (updateSchedContext ptr f)"
+  by (wpsimp simp: updateSchedContext_def obj_at'_def projectKOs opt_map_def)
+
+lemma update_sched_context_rewrite:
+  "monadic_rewrite False True (sc_obj_at n scp)
+    (update_sched_context scp f)
+      (do sc \<leftarrow> get_sched_context scp;
+          set_object scp (kernel_object.SchedContext (f sc) n) od)"
+  apply (clarsimp simp: update_sched_context_def get_sched_context_def bind_assoc)
+  apply (rule monadic_rewrite_bind_tail)
+   defer
+   apply (rule get_object_sp)
+  apply (case_tac obj;
+         fastforce simp: monadic_rewrite_refl3 set_object_def monadic_rewrite_def obj_at_def
+                         is_sc_obj_def)
+  done
+
+lemma updateSchedContext_corres_gen:
+  assumes
+      R1: "\<forall>s s'. (s, s') \<in> state_relation \<longrightarrow>
+           P s \<longrightarrow> P' s' \<longrightarrow> sc_at ptr s \<longrightarrow> sc_at' ptr s' \<longrightarrow>
+           (\<forall>n. (((\<lambda>ko. obj_bits ko = min_sched_context_bits + n) |< kheap s) ptr)\<longrightarrow>
+           sc_relation (the ((scs_of2 s ||> f) ptr)) n (the ((scs_of' s' ||> f') ptr)))"
+  and R2: "\<forall>s s'. (s, s') \<in> state_relation \<longrightarrow>
+          P s \<longrightarrow> P' s' \<longrightarrow> sc_at ptr s \<longrightarrow> sc_at' ptr s' \<longrightarrow>
+           heap_ls (replyPrevs_of s')  (scReply (the ((scs_of' s' ||> f') ptr)))
+             (sc_replies (the ((scs_of2 s ||> f) ptr)))"
+  and sz: "\<forall>sc'::sched_context. objBits sc' = objBits (f' sc')"
+  shows "corres dc
+         (sc_at ptr and P)
+         (sc_at' ptr and P')
+            (update_sched_context ptr f)
+            (updateSchedContext ptr f')"
+  unfolding corres_underlying_def using sz
+  apply clarsimp
+  apply (rename_tac s s')
+  apply (drule obj_at_ko_at)
+  apply (drule obj_at_ko_at')
+  apply (clarsimp simp: is_sc_obj)
+  apply (rename_tac sc' n sc)
+  apply (rule conjI, clarsimp)
+   apply (erule use_valid[OF _ updateSchedContext_wp])
+   apply clarsimp
+   apply (rule_tac x="((), s\<lparr>kheap := kheap s(ptr \<mapsto>
+                  kernel_object.SchedContext (f sc) n)\<rparr>)" in bexI)
+    apply clarsimp
+    apply (drule state_relation_sc_update[OF R1 R2 sz, simplified])
+      apply ((fastforce simp: obj_at_def is_sc_obj obj_at'_def projectKOs)+)[4]
+    apply (clarsimp simp: obj_at_def obj_at'_def projectKOs fun_upd_def[symmetric] opt_map_red)
+    apply (case_tac s; case_tac s'; fastforce)
+   apply (clarsimp simp: update_sched_context_def obj_at_def in_monad
+                         get_object_def set_object_def a_type_def)
+  apply (clarsimp intro!: no_failD[OF no_fail_updateSchedContext]
+                    simp: obj_at'_def projectKOs opt_map_def)
+  done
+
+lemmas updateSchedContext_corres = updateSchedContext_corres_gen[where P=\<top> and P'=\<top>, simplified]
+
+(* end : updateSchedContext *)
+
+end
+
+(* FIXME RT: rename *)
+(* this let us cross the sc size information from concrete to abstract *)
+lemma ko_at'_cross:
+  assumes p: "pspace_relation (kheap s) (ksPSpace s')"
+  assumes t: "ko_at' (sc'::sched_context) ptr s'"
+  shows "sc_obj_at (objBits sc' - minSchedContextBits) ptr s" using assms
+  apply (clarsimp simp: obj_at'_def projectKOs)
+  apply (erule (1) pspace_dom_relatedE)
+  by (clarsimp simp: obj_relation_cuts_def2 obj_at_def is_sc_obj cte_relation_def
+                     other_obj_relation_def pte_relation_def
+                     scBits_simps sc_relation_def objBits_simps
+              split: Structures_A.kernel_object.split_asm if_split_asm
+                     RISCV64_A.arch_kernel_obj.split_asm)
+
+lemma update_sc_no_reply_stack_update_ko_at'_corres:
+  assumes x: "\<And>sc n. sc_relation sc n sc' \<longrightarrow> sc_relation (f sc) n (f' sc')"
+  assumes y: "\<And>sc. sc_replies sc = sc_replies (f sc)"
+  assumes z: "objBits sc' = objBits (f' sc')"
+  assumes r: "scReply sc' = scReply (f' sc')"
+  shows
+    "corres dc (sc_at ptr) (ko_at' sc' ptr)
+            (update_sched_context ptr f)
+            (setSchedContext ptr (f' sc'))"
+  unfolding update_sched_context_def
+  apply (rule corres_guard_imp)
+    apply (rule corres_symb_exec_l'[where Q'="\<lambda>r s. ko_at r ptr s \<and> (\<exists>n. is_sc_obj n r)",
+                                    where P="\<lambda>s. obj_at \<top> ptr s"])
+      apply (rule corres_guard_imp[where P'=R and Q'=R for R])
+        apply (rule_tac F="(\<exists>n. is_sc_obj n obj)" in corres_gen_asm)
+        apply (case_tac obj; simp add: is_sc_obj_def)
+        apply (rule setSchedContext_no_stack_update_corres[where f'=f'])
+           apply (clarsimp simp: x obj_at_def intro!: y z r)+
+     apply (fastforce simp: exs_valid_def get_object_def in_monad)
+    apply (wpsimp wp: get_object_wp)
+   apply (fastforce simp: obj_at_def)
+  apply simp
+  done
+
+lemma update_sc_no_reply_stack_update_corres:
+  "\<lbrakk>\<forall>sc n sc'. sc_relation sc n sc' \<longrightarrow> sc_relation (f sc) n (f' sc');
+    \<forall>sc. sc_replies sc = sc_replies (f sc); \<forall>sc'. objBits sc' = objBits (f' sc');
+    \<forall>sc'. scReply (f' sc') = scReply sc' \<rbrakk> \<Longrightarrow>
+   corres dc (sc_at ptr and pspace_aligned and pspace_distinct) \<top>
+          (update_sched_context ptr f)
+         (do sc' <- getSchedContext ptr;
+             setSchedContext ptr (f' sc')
+          od)"
+  apply (rule_tac Q="sc_at' ptr" in corres_cross_add_guard)
+   apply (fastforce dest!: state_relationD sc_at_cross simp: obj_at'_def)
+  apply (rule corres_symb_exec_r)
+     apply (rule corres_guard1_imp)
+      apply (rule update_sc_no_reply_stack_update_ko_at'_corres; simp)
+     apply clarsimp
+    apply (wpsimp wp: get_sched_context_exs_valid simp: is_sc_obj_def obj_at_def)
+   apply (rename_tac ko; case_tac ko; simp)
+   apply (wpsimp simp: obj_at_def is_sc_obj_def)+
+  done
+
+lemma ko_at'_inj:
+  "ko_at' ko ptr  s \<Longrightarrow> ko_at' ko' ptr s \<Longrightarrow> ko' = ko"
+  by (clarsimp simp: obj_at'_real_def ko_wp_at'_def)
+
+(* FIXME RT: Move these to AInvs where possible *)
+(* FIXME RT: Try to unify with existing notions.
+             See https://sel4.atlassian.net/browse/VER-1382 *)
+definition injective_ref where
+  "injective_ref ref heap \<equiv> (\<forall>q p1 p2. (p1, ref) \<in> heap q \<and> (p2, ref) \<in> heap q \<longrightarrow> p1 = p2)"
+
+lemma sym_refs_inj:
+  "\<lbrakk>sym_refs heap; injective_ref (symreftype ref) heap; (x, ref) \<in> heap y; (x, ref) \<in> heap y'\<rbrakk>
+   \<Longrightarrow> y = y' "
+  apply (clarsimp simp: sym_refs_def injective_ref_def)
+  apply fastforce
+  done
+
+lemma sym_refs_inj2:
+  "\<lbrakk>sym_refs heap; injective_ref ref heap; (x, ref) \<in> heap y; (y, symreftype ref) \<in> heap z\<rbrakk>
+   \<Longrightarrow> x = z "
+  apply (subgoal_tac "(y, symreftype ref) \<in> heap x")
+   apply (erule (3) sym_refs_inj[where ref="symreftype ref", simplified])
+  apply (fastforce simp: sym_refs_def)
+  done
+
+lemma injective_ref_SCTcb[simp]:
+  "injective_ref SCTcb (state_refs_of' s) "
+  apply (clarsimp simp: state_refs_of'_def injective_ref_def split: option.splits if_splits)
+  apply (clarsimp simp: refs_of'_def)
+  apply (rename_tac p0 ko p1 p2)
+  apply (prop_tac "\<exists>z. ko = KOSchedContext z")
+   apply (clarsimp split: kernel_object.splits)
+      apply (clarsimp split: Structures_H.endpoint.splits simp: ep_q_refs_of'_def)
+     apply (clarsimp split: Structures_H.ntfn.splits option.splits
+                      simp: ntfn_q_refs_of'_def get_refs_def)
+    apply (clarsimp simp: tcb_st_refs_of'_def tcb_bound_refs'_def get_refs_def
+                   split: Structures_H.thread_state.splits if_splits option.splits)
+   apply (clarsimp simp: get_refs_def split: option.splits)
+  apply (clarsimp simp: get_refs_def split: option.splits)
+  done
+
+lemma reply_at'_cross_rel:
+  "cross_rel (pspace_aligned and pspace_distinct and reply_at t) (reply_at' t)"
+  unfolding cross_rel_def state_relation_def
+  apply clarsimp
+  by (erule (3) reply_at_cross)
+
+lemma sch_act_simple_cross_rel:
+  "cross_rel simple_sched_action sch_act_simple"
+  apply (clarsimp simp: cross_rel_def)
+  by (fastforce simp: simple_sched_action_def sch_act_simple_def
+                dest: state_relation_sched_act_relation
+               split: Structures_A.scheduler_action.splits)
+
+(* FIXME RT: move to Corres_UL.thy *)
+lemma cross_relF:
+  "(s, s') \<in> state_relation \<Longrightarrow> cross_rel A B \<Longrightarrow> A s \<Longrightarrow> B s'"
+  by (clarsimp simp: cross_rel_def)
+
+lemma valid_tcb_state'_simps[simp]:
+  "valid_tcb_state' Running = \<top>"
+  "valid_tcb_state' Inactive = \<top>"
+  "valid_tcb_state' Restart = \<top>"
+  "valid_tcb_state' IdleThreadState = \<top>"
+  "valid_tcb_state' (BlockedOnSend ref b c d e) = ep_at' ref"
+  "valid_tcb_state' (BlockedOnReply r) = valid_bound_reply' r"
+  by (rule ext, simp add: valid_tcb_state'_def)+
+
+lemma tcb_at'_ex1_ko_at':
+  "tcb_at' t s \<Longrightarrow> \<exists>!tcb. ko_at' (tcb::tcb) t s"
+  by (clarsimp simp: obj_at'_def)
+
+lemma ex1_ex_eq_all:
+  "\<exists>!x. Q x \<Longrightarrow> (\<exists>x. Q x \<and> P x) = (\<forall>x. Q x \<longrightarrow> P x)"
+  by fastforce
+
+lemmas tcb_at'_ex_eq_all = ex1_ex_eq_all[OF tcb_at'_ex1_ko_at']
+
+lemma receiveBlocked_equiv:
+  "receiveBlocked st = is_BlockedOnReceive st"
+  unfolding receiveBlocked_def
+  by (case_tac st; simp)
+
+lemma threadGet_getObject:
+  "threadGet f t = do x <- getObject t;
+                         return (f x)
+                   od"
+  apply (simp add: threadGet_def threadRead_def oliftM_def getObject_def[symmetric])
+  done
+
+lemma obj_at'_typ_at'[elim!]:
+  "obj_at' (P :: ('a :: pspace_storable) \<Rightarrow> bool) p s \<Longrightarrow>
+   obj_at' (\<top> :: ('a :: pspace_storable) \<Rightarrow> bool) p s"
+  by (clarsimp simp: obj_at'_real_def ko_wp_at'_def)
+
+lemma shows
+  obj_at'_sc_tcbs_of_equiv:
+    "obj_at' (\<lambda>x. scTCB x = Some t) p s = (sc_at' p s \<and> scTCBs_of s p = Some t)"
+  and obj_at'_tcb_scs_of_equiv:
+    "obj_at' (\<lambda>x. tcbSchedContext x = Some sc) p s = (tcb_at' p s \<and> tcbSCs_of s p = Some sc)"
+  and obj_at'_replySCs_of_equiv:
+    "obj_at' (\<lambda>a. replyNext a = Some (Head sc)) p s = (reply_at' p s \<and> replySCs_of s p = Some sc)"
+  and obj_at'_scReplies_of_equiv:
+    "obj_at' (\<lambda>a. scReply a = Some sc) p s = (sc_at' p s \<and> scReplies_of s p = Some sc)"
+  by (intro iffI; clarsimp simp: obj_at'_real_def ko_wp_at'_def projectKOs opt_map_def)+
+
+lemma not_idle_scTCB:
+  "\<lbrakk>sym_heap_tcbSCs s; valid_objs' s; valid_idle' s; p \<noteq> idle_sc_ptr; sc_at' p s\<rbrakk> \<Longrightarrow>
+   obj_at' (\<lambda>x. scTCB x \<noteq> Some idle_thread_ptr) p s"
+  apply (subgoal_tac "\<not>obj_at' (\<lambda>x. scTCB x = Some idle_thread_ptr) p s")
+   apply (clarsimp simp: obj_at'_real_def ko_wp_at'_def)
+  apply (subst (asm) sym_heap_symmetric)
+  apply (clarsimp simp: obj_at'_sc_tcbs_of_equiv sym_heap_def)
+  apply (clarsimp simp: valid_idle'_def obj_at'_real_def ko_wp_at'_def idle_tcb'_def projectKOs)
+  done
+
+lemma not_idle_tcbSC:
+  "\<lbrakk>sym_heap_tcbSCs s; valid_objs' s; valid_idle' s; p \<noteq> idle_thread_ptr; tcb_at' p s\<rbrakk> \<Longrightarrow>
+   obj_at' (\<lambda>x. tcbSchedContext x \<noteq> Some idle_sc_ptr) p s"
+  apply (subgoal_tac "\<not>obj_at' (\<lambda>x. tcbSchedContext x = Some idle_sc_ptr) p s")
+   apply (clarsimp simp: obj_at'_real_def ko_wp_at'_def)
+  apply (clarsimp simp: obj_at'_tcb_scs_of_equiv sym_heap_def)
+  apply (clarsimp simp: valid_idle'_def obj_at'_real_def ko_wp_at'_def idle_tcb'_def projectKOs)
+  done
+
+lemma setObject_tcb_tcbs_of':
+  "\<lbrace>\<lambda>s. P' ((tcbs_of' s)(c \<mapsto> tcb))\<rbrace>
+  setObject c (tcb::tcb)
+  \<lbrace>\<lambda>_ s. P' (tcbs_of' s)\<rbrace>"
+  by (setObject_easy_cases, clarsimp simp: RISCV64_H.fromPPtr_def)
+
+lemma setObject_other_tcbs_of'[wp]:
+  "setObject c (r::reply) \<lbrace>\<lambda>s. P' (tcbs_of' s)\<rbrace>"
+  "setObject c (e::endpoint) \<lbrace>\<lambda>s. P' (tcbs_of' s)\<rbrace>"
+  "setObject c (n::notification) \<lbrace>\<lambda>s. P' (tcbs_of' s)\<rbrace>"
+  "setObject c (sc::sched_context) \<lbrace>\<lambda>s. P' (tcbs_of' s)\<rbrace>"
+  by setObject_easy_cases+
+
+lemma setObject_cte_tcbSCs_of[wp]:
+  "setObject c (reply::cte) \<lbrace>\<lambda>s. P' (tcbSCs_of s)\<rbrace>"
+  by setObject_easy_cases
+
+lemma threadSet_tcbSCs_of_inv:
+  "\<forall>x. tcbSchedContext (f x) = tcbSchedContext x \<Longrightarrow>
+  threadSet f t \<lbrace>\<lambda>s. P (tcbSCs_of s)\<rbrace>"
+  unfolding threadSet_def
+  apply (rule hoare_seq_ext[OF _ get_tcb_sp'])
+  apply (wpsimp wp: setObject_tcb_tcbs_of')
+  apply (erule subst[where P=P, rotated], rule ext)
+  apply (clarsimp simp: opt_map_def obj_at'_real_def ko_wp_at'_def projectKO_tcb
+                 split: option.splits)
+  done
+
+lemma aligned'_distinct'_obj_at'I:
+  "\<lbrakk> \<exists>y. ksPSpace s p = Some (injectKO (y:: 'a::pspace_storable));
+    pspace_aligned' s; pspace_distinct' s;
+    (if koTypeOf (the (ksPSpace s p))  = SchedContextT then pspace_bounded' s else True)\<rbrakk>
+   \<Longrightarrow> obj_at' (\<top> :: 'a::pspace_storable \<Rightarrow> bool) p s"
+  apply (clarsimp)
+  apply (frule_tac v=y in aligned'_distinct'_ko_at'I; simp?)
+  apply (case_tac "injectKO y"; clarsimp simp: valid_sz_simps dest!: pspace_boundedD')
+  done
+
+(* FIXME RT: maybe move? *)
+lemma prod_in_refsD:
+  "\<And>ref x y. (x, ref) \<in> ep_q_refs_of' y \<Longrightarrow> ref \<in> {EPRecv, EPSend}"
+  "\<And>ref x y. (x, ref) \<in> ntfn_q_refs_of' y \<Longrightarrow> ref \<in> {NTFNSignal}"
+  "\<And>ref x y. (x, ref) \<in> tcb_st_refs_of' y \<Longrightarrow> ref \<in> {TCBBlockedRecv, TCBReply, TCBSignal, TCBBlockedSend}"
+  "\<And>ref x a b c. (x, ref) \<in> tcb_bound_refs' a b c \<Longrightarrow> ref \<in> {TCBBound, TCBSchedContext, TCBYieldTo}"
+  apply (rename_tac ep; case_tac ep; simp)
+  apply (rename_tac ep; case_tac ep; simp)
+  apply (rename_tac ep; case_tac ep; clarsimp split: if_splits)
+  apply (clarsimp simp: tcb_bound_refs'_def get_refs_def2)
+  done
+
+lemma sym_refs_tcbSCs:
+  "\<lbrakk>sym_refs (state_refs_of' s); pspace_aligned' s; pspace_distinct' s; pspace_bounded' s\<rbrakk>
+   \<Longrightarrow> sym_heap_tcbSCs s"
+  apply (clarsimp simp: sym_heap_def)
+  apply (rule iffI)
+   apply (drule_tac tp=SCTcb and x=p and y=p' in sym_refsE;
+          force simp: get_refs_def2 state_refs_of'_def projectKOs opt_map_red refs_of_rev'
+                dest: pspace_alignedD' pspace_distinctD' pspace_boundedD' split: if_split_asm option.split_asm)+
+  by (drule_tac tp=TCBSchedContext and x=p' and y=p in sym_refsE;
+      force simp: get_refs_def2 state_refs_of'_def projectKOs opt_map_red refs_of_rev'
+               dest: pspace_alignedD' pspace_distinctD' pspace_boundedD' split: if_split_asm option.split_asm)+
+
+lemma sym_refs_scReplies:
+  "\<lbrakk>sym_refs (state_refs_of' s); pspace_aligned' s; pspace_distinct' s; pspace_bounded' s\<rbrakk>
+   \<Longrightarrow> sym_heap_scReplies s"
+  apply (clarsimp simp: sym_heap_def)
+  apply (rule iffI)
+   apply (drule_tac tp=ReplySchedContext and x=p and y=p' in sym_refsE;
+          force simp: get_refs_def2 state_refs_of'_def projectKOs opt_map_red refs_of_rev'
+                dest: pspace_alignedD' pspace_distinctD' pspace_boundedD' split: if_split_asm option.split_asm)+
+  by (drule_tac tp=SCReply and x=p' and y=p in sym_refsE;
+      force simp: get_refs_def2 state_refs_of'_def projectKOs opt_map_red refs_of_rev'
+               dest: pspace_alignedD' pspace_distinctD' pspace_boundedD' split: if_split_asm option.split_asm)+
+
+lemma setSchedContext_scTCBs_of:
+  "\<lbrace>\<lambda>s. P (\<lambda>a. if a = scPtr then scTCB sc else scTCBs_of s a)\<rbrace>
+   setSchedContext scPtr sc
+   \<lbrace>\<lambda>_ s. P (scTCBs_of s)\<rbrace>"
+  unfolding setSchedContext_def
+  apply (wpsimp wp: setObject_sc_wp)
+  apply (erule back_subst[where P=P], rule ext)
+  by (clarsimp simp: opt_map_def)
+
+lemma setSchedContext_scReplies_of:
+  "\<lbrace>\<lambda>s. P (\<lambda>a. if a = scPtr then scReply sc else scReplies_of s a)\<rbrace>
+   setSchedContext scPtr sc
+   \<lbrace>\<lambda>_ s. P (scReplies_of s)\<rbrace>"
+  unfolding setSchedContext_def
+  apply (wpsimp wp: setObject_sc_wp)
+  apply (erule back_subst[where P=P], rule ext)
+  by (clarsimp simp: opt_map_def)
+
+lemma getObject_tcb_wp:
+  "\<lbrace>\<lambda>s. tcb_at' p s \<longrightarrow> (\<exists>t::tcb. ko_at' t p s \<and> Q t s)\<rbrace> getObject p \<lbrace>Q\<rbrace>"
+  by (clarsimp simp: getObject_def valid_def in_monad
+                     split_def objBits_simps' loadObject_default_def
+                     projectKOs obj_at'_def in_magnitude_check
+              dest!: readObject_misc_ko_at')
+
+
+lemma threadSet_tcbSCs_of:
+  "\<lbrace>\<lambda>s. P (\<lambda>a. if a = t then tcbSchedContext (f (the (tcbs_of' s a))) else tcbSCs_of s a)\<rbrace>
+   threadSet f t
+   \<lbrace>\<lambda>_ s. P (tcbSCs_of s)\<rbrace>"
+  unfolding threadSet_def
+  apply (wpsimp wp: setObject_tcb_wp getObject_tcb_wp)
+  apply (clarsimp simp: tcb_at'_ex_eq_all)
+  apply (erule back_subst[where P=P], rule ext)
+  apply (clarsimp simp: opt_map_def obj_at'_real_def ko_wp_at'_def projectKOs)
+  done
+
+lemma shows
+  replyNexts_Some_replySCs_None:
+  "replyNexts_of s rp \<noteq> None \<Longrightarrow> replySCs_of s rp = None" and
+  replySCs_Some_replyNexts_None:
+  "replySCs_of s rp \<noteq> None \<Longrightarrow> replyNexts_of s rp = None"
+  by (clarsimp simp: opt_map_def projectKOs split: option.splits reply_next.splits)+
+
+lemma sym_heap_remove_only:
+  "\<lbrakk> sym_heap h1 h2; h2 y = Some x \<rbrakk> \<Longrightarrow>
+   sym_heap (\<lambda>a. if a = x then None else h1 a) (\<lambda>a. if a = y then None else h2 a)"
+  supply opt_mapE [rule del]
+  apply (clarsimp simp: sym_heap_def)
+  apply (subst (asm) sym_heap_symmetric[simplified sym_heap_def], simp)
+  done
+
+lemma pred_tcb_at'_equiv:
+  "pred_tcb_at' p P t s = (tcb_at' t s \<and> P (p (tcb_to_itcb' (the (tcbs_of' s t)))))"
+  by (rule iffI;
+      clarsimp simp: pred_tcb_at'_def pred_map_def obj_at'_real_def ko_wp_at'_def projectKOs
+                     opt_map_def)
+
+lemma isBlockedOnSend_equiv:
+  "isBlockedOnSend st = is_BlockedOnSend st"
+  by (case_tac st; simp add: isBlockedOnSend_def)
+
+lemma isSend_equiv:
+  "isSend st = is_BlockedOnSend st"
+  by (case_tac st; simp add: isSend_def)
+
+lemma sch_act_wf_not_runnable_sch_act_not:
+  "\<lbrakk>st_tcb_at' P t s; sch_act_wf (ksSchedulerAction s) s; \<forall>st. P st \<longrightarrow> \<not> runnable' st\<rbrakk> \<Longrightarrow>
+   sch_act_not t s"
+   by (clarsimp simp: pred_tcb_at'_def obj_at'_def)
+
+lemma isTimeoutFault_fault_map[simp]:
+  "isTimeoutFault (fault_map a) = is_timeout_fault a"
+  by (clarsimp simp: isTimeoutFault_def fault_map_def is_timeout_fault_def
+              split: ExceptionTypes_A.fault.splits)
+
+lemma valid_bound_obj_lift:
+  "f \<lbrace>P (the x)\<rbrace> \<Longrightarrow> f \<lbrace>valid_bound_obj P x\<rbrace>"
+  unfolding valid_bound_obj_def
+  by (case_tac x; wpsimp)
+
+lemma valid_bound_obj'_lift:
+  "f \<lbrace>P (the x)\<rbrace> \<Longrightarrow> f \<lbrace>valid_bound_obj' P x\<rbrace>"
+  unfolding valid_bound_obj'_def
+  by (case_tac x; wpsimp)
+
+lemma ep_at'_cross_rel:
+  "cross_rel (pspace_aligned and pspace_distinct and ep_at t) (ep_at' t)"
+  unfolding cross_rel_def state_relation_def
+  apply clarsimp
+  by (erule (3) ep_at_cross)
+
+lemma sch_act_not_cross_rel:
+  "cross_rel (scheduler_act_not t) (sch_act_not t)"
+  unfolding cross_rel_def state_relation_def
+  apply clarsimp
+  apply (case_tac "scheduler_action s"; simp)
+  by (clarsimp simp: scheduler_act_not_def sched_act_relation_def)
+
+global_interpretation set_simple_ko: typ_at_pres "set_simple_ko C ptr ep"
+  unfolding typ_at_pres_def by wpsimp
+
+global_interpretation update_sk_obj_ref: typ_at_pres "update_sk_obj_ref C update ref new"
+  unfolding typ_at_pres_def by wpsimp
+
+lemma getReprogramTimer_corres:
+  "corres (=) \<top> \<top> (gets reprogram_timer) getReprogramTimer"
+  by (clarsimp simp: getReprogramTimer_def state_relation_def)
+
+lemma setDomainTime_corres:
+  "dt = dt' \<Longrightarrow>
+  corres dc \<top> \<top> (modify (domain_time_update (\<lambda>_. dt))) (setDomainTime dt')"
+  apply (clarsimp simp: setDomainTime_def, rule corres_modify)
+  by (clarsimp simp: state_relation_def swp_def)
+
+lemma setConsumedTime_corres:
+  "ct = ct' \<Longrightarrow>
+  corres dc \<top> \<top> (modify (consumed_time_update (\<lambda>_. ct))) (setConsumedTime ct')"
+  apply (clarsimp simp: setConsumedTime_def, rule corres_modify)
+  by (clarsimp simp: state_relation_def swp_def)
+
+lemma setCurSc_corres:
+  "sc = sc' \<Longrightarrow>
+   corres dc \<top> \<top> (modify (cur_sc_update (\<lambda>_. sc))) (setCurSc sc')"
+  apply (clarsimp simp: setCurSc_def, rule corres_modify)
+  by (clarsimp simp: state_relation_def swp_def)
+
+lemma refillSingle_equiv:
+  "sc_valid_refills' sc \<Longrightarrow>
+   (length (refills_map (scRefillHead sc) (scRefillCount sc) (scRefillMax sc) (scRefills sc)) = Suc 0)
+    = (scRefillHead sc = refillTailIndex sc)"
+  apply (clarsimp simp: valid_sched_context'_def refillTailIndex_def refills_map_def)
+  apply (case_tac "scRefillCount sc = Suc 0"; simp)
+  apply (auto simp: Let_def)
+  done
+
+lemma refillSingle_corres:
+  "scp = scp' \<Longrightarrow>
+   corres (=) (sc_at scp) (obj_at' sc_valid_refills' scp')
+     (refill_single scp)
+     (refillSingle scp')"
+  unfolding refill_single_def refillSingle_def
+  apply (simp add: refill_size_def get_refills_def)
+  apply (rule stronger_corres_guard_imp)
+    apply (rule_tac R'="\<lambda>sc s. sc_valid_refills' sc" and R="\<lambda>_ _ . True" in corres_split)
+       apply (rule get_sc_corres)
+      apply simp
+      apply (metis (mono_tags, hide_lams) refillSingle_equiv sc_relation_def)
+     apply wpsimp+
+  apply (clarsimp simp: obj_at'_def)
+  done
+
+lemma active_sc_at'_cross:
+  "\<lbrakk>(s,s') \<in> state_relation; pspace_aligned s; pspace_distinct s; is_active_sc sc_ptr s;
+    sc_at sc_ptr s\<rbrakk>
+   \<Longrightarrow> active_sc_at' sc_ptr s'"
+  apply (frule state_relation_pspace_relation)
+  apply (frule (3) sc_at_cross)
+  apply (clarsimp simp: pspace_relation_def obj_at_def is_sc_obj_def)
+  apply (drule_tac x=sc_ptr in bspec, blast)
+  apply (clarsimp simp: sc_relation_def vs_all_heap_simps active_sc_at'_def obj_at'_def projectKOs
+                        active_sc_def)
+  done
+
+lemma is_active_sc'2_cross:
+  "\<lbrakk>(s,s') \<in> state_relation; pspace_aligned s; pspace_distinct s; is_active_sc sc_ptr s;
+    sc_at sc_ptr s\<rbrakk>
+   \<Longrightarrow> is_active_sc' sc_ptr s'"
+  apply (frule state_relation_pspace_relation)
+  apply (frule (3) sc_at_cross)
+  apply (clarsimp simp: pspace_relation_def obj_at_def is_sc_obj_def)
+  apply (drule_tac x=sc_ptr in bspec, blast)
+  apply (clarsimp simp: sc_relation_def vs_all_heap_simps obj_at'_def projectKOs
+                        active_sc_def opt_map_red StateRelation.is_active_sc'_def)
+  done
+
+\<comment> \<open>Some methods to add invariants to the concrete guard of a corres proof. Often used for properties
+    that are asserted to hold in the Haskell definition.\<close>
+
+method add_sym_refs =
+  rule_tac Q="\<lambda>s'. sym_refs (state_refs_of' s')" in corres_cross_add_guard,
+  (clarsimp simp: pred_conj_def)?,
+  (elim conjE)?,
+  (frule invs_sym_refs)?, (frule invs_psp_aligned)?, (frule invs_distinct)?,
+  fastforce dest: state_refs_of_cross_eq
+
+method add_ct_not_inQ =
+  rule_tac Q="\<lambda>s'. ct_not_inQ s'" in corres_cross_add_guard,
+  fastforce intro!: ct_not_inQ_cross simp: valid_sched_def
+
+method add_sch_act_wf =
+  rule_tac Q="\<lambda>s'. sch_act_wf (ksSchedulerAction s') s'" in corres_cross_add_guard,
+  fastforce intro!: sch_act_wf_cross simp: valid_sched_def
+
+method add_ct_idle_or_in_cur_domain' =
+  rule_tac Q="\<lambda>s'. ct_idle_or_in_cur_domain' s'" in corres_cross_add_guard,
+  fastforce intro!: ct_idle_or_in_cur_domain'_cross simp: valid_sched_def
+
+method add_valid_idle' =
+  rule_tac Q="\<lambda>s'. valid_idle' s'" in corres_cross_add_guard,
+  fastforce intro!: valid_idle'_cross
+
+method add_ready_qs_runnable =
+  rule_tac Q=ready_qs_runnable in corres_cross_add_guard,
+  (clarsimp simp: pred_conj_def)?,
+  (frule valid_sched_valid_ready_qs)?, (frule invs_psp_aligned)?, (frule invs_distinct)?,
+  fastforce dest: ready_qs_runnable_cross
+
+method add_valid_replies for rptr uses simp =
+  rule_tac Q="\<lambda>s. valid_replies'_sc_asrt rptr s" in corres_cross_add_guard,
+  fastforce elim: valid_replies_sc_cross simp: simp
+
 end
